further cleanup on names and proof order/structure

theories/eps0.v
@@ -63,10 +63,14 @@ Set Implicit Arguments.
 #[global] Reserved Notation "e '<ε₀' f" (at level 70, format "e  <ε₀  f").
 #[global] Reserved Notation "e '≤ε₀' f" (at level 70, format "e  ≤ε₀  f").
 
+#[global] Reserved Notation "a '+₀' b"  (at level 31, left associativity, format "a  +₀  b" ).
+#[global] Reserved Notation "a '*₀' b"  (at level 29, left associativity, format "a  *₀  b" ).
+#[global] Reserved Notation "'ω^' e" (at level 1, format "ω^ e").
+#[global] Reserved Notation "'ω^⟨' e , i '⟩'" (at level 0, format "ω^⟨ e , i ⟩").
+
 #[local] Hint Constructors clos_trans : core.
-#[local] Hint Resolve Acc_inv Acc_intro 
-                      in_cons in_eq in_elt in_or_app : core.
 #[local] Hint Resolve clos_trans_rev transitive_rev : core.
+#[local] Hint Resolve in_cons in_eq in_elt in_or_app : core.
 #[local] Hint Constructors lex2 : core.
 
 (** ε₀ is the sub-type of E0 composed of trees in nested lexigraphic order *)
@@ -126,7 +130,7 @@ Section eps0_order.
   Fact wf_eps0_lt : well_founded eps0_lt.
   Proof.
     generalize E0_lt_wf.
-    apply wf_rel_morph with (f := fun x y => x = π₁ y).
+    apply wf_rel_morph with (f := λ x y, x = π₁ y).
     + intros []; eauto.
     + unfold eps0_lt; intros ? ? [] [] -> ->; simpl; eauto.
   Qed.
@@ -251,7 +255,9 @@ Arguments eps0_lt /.
              eps0_le_refl eps0_le_antisym
              eps0_lt_trans eps0_le_trans 
              eps0_le_lt_trans
-             eps0_lt_le_trans : core.
+             eps0_lt_le_trans
+             eps0_lt_succ
+             eps0_le_not_succ : core.
 
 #[global] Infix "<ε₀" := eps0_lt.
 #[global] Infix "≤ε₀" := eps0_le.
@@ -262,7 +268,7 @@ Arguments eps0_lt /.
 Theorem eps0_rect (P : ε₀ → Type) : (∀f, (∀e, e <ε₀ f → P e) → P f) → ∀e, P e.
 Proof. apply (well_founded_induction_type wf_eps0_lt). Qed.
 
-Section eps0_add.
+Section eps0_add_base.
 
   Hint Resolve E0_add_cnf : core.
 
@@ -302,7 +308,13 @@ Section eps0_add.
   Fact eps0_add_mono_right : ∀ e f g, f <ε₀ g → e +₀ f <ε₀ e +₀ g.
   Proof. intros [] [] []; simpl; apply E0_add_mono_right; auto. Qed.
 
-  Hint Resolve eps0_add_mono_left eps0_add_mono_right : core.
+End eps0_add_base.
+
+#[global] Infix "+₀" := eps0_add.
+
+#[local] Hint Resolve eps0_add_mono_left eps0_add_mono_right : core.
+
+Section eps0_add_extra.
 
   Fact eps0_add_mono e e' f f' : e ≤ε₀ e' → f ≤ε₀ f' → e +₀ f ≤ε₀ e' +₀ f'.
   Proof. intros ? [ | <- ]; eauto. Qed.
@@ -412,7 +424,7 @@ Section eps0_add.
   Fact eps0_add_le_cancel e u v : e +₀ u ≤ε₀ e +₀ v → u ≤ε₀ v.
   Proof. now intros [ ?%eps0_add_lt_cancel | ?%eps0_add_cancel ]; [ left | right ]. Qed.
 
-End eps0_add.
+End eps0_add_extra.
 
 #[global] Infix "+₀" := eps0_add.
 
@@ -430,95 +442,98 @@ End eps0_add.
 
 Section eps0_omega.
 
-  (* ω^{e.(S n)} *)
-  Definition eps0_exp_S : ε₀ → pos → ε₀.
+  Hint Resolve cnf_sg : core.
+
+  (* ω^e.p where p is positive *)
+  Definition eps0_exp : ε₀ → pos → ε₀.
   Proof.
-    intros (e & He) n.
-    exists (E0_cons [(e,n)]).
-    now apply cnf_sg.
+    intros (e & He) p.
+    exists (E0_cons [(e,p)]); auto.
   Defined.
 
-  (* Beware that this is for ωᵉ.(1+i) and NOT ωᵉ.i *)
-  Notation "ω^⟨ e , i ⟩" := (eps0_exp_S e i).
+  Notation "ω^⟨ e , i ⟩" := (eps0_exp e i).
 
-  Fact eps0_succ_exp_S n : S₀ ω^⟨0₀,n⟩ = ω^⟨0₀,n +ₚ 1ₚ⟩.
+  Fact eps0_succ_exp n : S₀ ω^⟨0₀,n⟩ = ω^⟨0₀,n +ₚ 1ₚ⟩.
   Proof. apply eps0_eq_iff; simpl; apply E0_succ_pos. Qed.
 
-  Fact eps0_lt_exp_S e n : e <ε₀ ω^⟨e,n⟩.
+  Fact eps0_lt_exp : ∀ e n, e <ε₀ ω^⟨e,n⟩.
   Proof.
-    destruct e as [e]; unfold eps0_exp_S; cbn.
+    intros [] n; unfold eps0_exp; cbn.
     apply E0_lt_sub with n; auto.
-    apply cnf_sg; auto.
   Qed.
 
-  Fact eps0_lt_zero_exp_S e n : 0₀ <ε₀ ω^⟨e,n⟩.
-  Proof. apply eps0_le_lt_trans with (2 := eps0_lt_exp_S _ _); auto. Qed.
-
-  Hint Resolve eps0_lt_zero_exp_S : core.
-
-  Fact eps0_zero_neq_exp_S e n : 0₀ ≠ ω^⟨e,n⟩.
-  Proof.
-    intros E; apply (@eps0_lt_irrefl 0₀).
-    rewrite E at 2; apply eps0_lt_zero_exp_S.
-  Qed.
-
-  Fact eps0_exp_S_mono_right : ∀ e n m, n < m → ω^⟨e,n⟩ <ε₀ ω^⟨e,m⟩.
+  Fact eps0_exp_mono_right : ∀ e n m, n < m → ω^⟨e,n⟩ <ε₀ ω^⟨e,m⟩.
   Proof. intros [] ? ?; simpl; constructor; constructor 2; right; auto. Qed.
 
-  Fact eps0_exp_S_mono_left : ∀ e f n m, e <ε₀ f → ω^⟨e,n⟩ <ε₀ ω^⟨f,m⟩.
+  Fact eps0_exp_mono_left : ∀ e f n m, e <ε₀ f → ω^⟨e,n⟩ <ε₀ ω^⟨f,m⟩.
   Proof. intros [] [] ? ?; apply E0_lt_exp. Qed.
 
-  Fact eps0_exp_S_mono e f n m : e ≤ε₀ f → n ≤ m → ω^⟨e,n⟩ ≤ε₀ ω^⟨f,m⟩.
+  Fact eps0_add_exp : ∀ e i j, ω^⟨e,i⟩ +₀ ω^⟨e,j⟩ = ω^⟨e,i +ₚ j⟩.
   Proof.
-    intros [ | <- ] H2.
-    + now left; apply eps0_exp_S_mono_left.
-    + destruct H2; auto.
-      left; apply eps0_exp_S_mono_right; lia.
-  Qed.
-
-  Fact eps0_exp_S_mono_inv e f n m : ω^⟨e,n⟩ <ε₀ ω^⟨f,m⟩ → e <ε₀ f ∨ e = f ∧ n < m.
-  Proof.
-    intros H.
-    destruct (eps0_lt_sdec e f) as [ | e | e f H1 ]; auto.
-    + destruct (lt_sdec n m) as [ | n | n m H2 ]; auto.
-      * contradict H; apply eps0_lt_irrefl.
-      * destruct (@eps0_lt_irrefl ω^⟨e,n⟩).
-        apply eps0_lt_trans with (1 := H).
-        now apply eps0_exp_S_mono_right.
-    + destruct (@eps0_lt_irrefl ω^⟨e,n⟩).
-      apply eps0_lt_trans with (1 := H).
-      now apply eps0_exp_S_mono_left.
-  Qed.
-  
-  Fact eps0_exp_S_inj e f n m : ω^⟨e,n⟩ = ω^⟨f,m⟩ → e = f ∧ n = m.
-  Proof.
-    intros E.
-    destruct (eps0_lt_sdec e f) as [ e f H | e | e f H ].
-    + apply eps0_exp_S_mono_left with (n := n) (m := m) in H.
-      rewrite E in H; now apply eps0_lt_irrefl in H.
-    + destruct (lt_sdec n m) as [ n m H | | n m H ]; auto;
-        apply eps0_exp_S_mono_right with (e := e) in H;
-        rewrite E in H; now apply eps0_lt_irrefl in H.
-    + apply eps0_exp_S_mono_left with (n := m) (m := n) in H.
-      rewrite E in H; now apply eps0_lt_irrefl in H.
-  Qed.
-
-  Fact eps0_add_exp_S e i j : ω^⟨e,i⟩ +₀ ω^⟨e,j⟩ = ω^⟨e,i +ₚ j⟩.
-  Proof.
-    destruct e as (e & He).
-    apply eps0_eq_iff; unfold eps0_add, eps0_exp_S, proj1_sig.
+    intros [] ? ?.
+    apply eps0_eq_iff; unfold eps0_add, eps0_exp, proj1_sig.
     rewrite E0_add_exp; do 3 f_equal.
   Qed.
 
-  Fact eps0_zero_neq_exp_S_add e n f: 0₀ ≠ ω^⟨e,n⟩ +₀ f.
+  (***********************)
+
+  Fact eps0_lt_zero_exp e n : 0₀ <ε₀ ω^⟨e,n⟩.
+  Proof. apply eps0_le_lt_trans with (2 := eps0_lt_exp _ _); auto. Qed.
+
+  Hint Resolve eps0_lt_zero_exp : core.
+
+  Fact eps0_zero_neq_exp e n : 0₀ ≠ ω^⟨e,n⟩.
+  Proof.
+    intros E; apply (@eps0_lt_irrefl 0₀).
+    rewrite E at 2; apply eps0_lt_zero_exp.
+  Qed.
+
+  Hint Resolve eps0_exp_mono_left eps0_exp_mono_right : core.
+
+  Fact eps0_exp_mono e f n m : e ≤ε₀ f → n ≤ m → ω^⟨e,n⟩ ≤ε₀ ω^⟨f,m⟩.
+  Proof.
+    intros [ H1 | <- ] H2; auto.
+    apply pos_le_lt_iff in H2 as [ <- | ]; auto.
+  Qed.
+
+  Hint Resolve eps0_exp_mono : core.
+
+  Fact eps0_exp_mono_inv e f n m : ω^⟨e,n⟩ <ε₀ ω^⟨f,m⟩ → e <ε₀ f ∨ e = f ∧ n < m.
+  Proof.
+    intros H.
+    destruct (eps0_lt_sdec e f) as [ | e | e f H1 ]; auto.
+    + destruct (pos_lt_sdec n m) as [ | n | n m H2 ]; auto.
+      * contradict H; apply eps0_lt_irrefl.
+      * destruct (@eps0_lt_irrefl ω^⟨e,n⟩).
+        apply eps0_lt_trans with (1 := H); auto.
+    + destruct (@eps0_lt_irrefl ω^⟨e,n⟩).
+      apply eps0_lt_trans with (1 := H); auto.
+  Qed.
+  
+  Fact eps0_exp_inj e f n m : ω^⟨e,n⟩ = ω^⟨f,m⟩ → e = f ∧ n = m.
+  Proof.
+    intros E.
+    destruct (eps0_lt_sdec e f) as [ e f H | e | e f H ].
+    + apply eps0_exp_mono_left with (n := n) (m := m) in H.
+      rewrite E in H; now apply eps0_lt_irrefl in H.
+    + destruct (pos_lt_sdec n m) as [ n m H | | n m H ]; auto;
+        apply eps0_exp_mono_right with (e := e) in H;
+        rewrite E in H; now apply eps0_lt_irrefl in H.
+    + apply eps0_exp_mono_left with (n := m) (m := n) in H.
+      rewrite E in H; now apply eps0_lt_irrefl in H.
+  Qed.
+
+(*
+  Fact eps0_zero_neq_exp_add e n f: 0₀ ≠ ω^⟨e,n⟩ +₀ f.
   Proof.
     intros H.
     apply (@eps0_lt_irrefl 0₀).
     rewrite H at 2.
-    apply eps0_lt_le_trans with (1 := eps0_lt_zero_exp_S e n).
+    apply eps0_lt_le_trans with (1 := eps0_lt_zero_exp e n).
     rewrite <- (eps0_add_zero_right ω^⟨e,n⟩) at 1.
     apply eps0_add_mono; auto.
   Qed.
+*)
 
   (* ωᵉ = ωᵉ.(1+0) *)
   Definition eps0_omega (e : ε₀) := ω^⟨e,1ₚ⟩.
@@ -527,58 +542,42 @@ Section eps0_omega.
   Fact eps0_omega_zero : ω^0₀ = 1₀.
   Proof. apply eps0_eq_iff; trivial. Qed.
 
-  Fact eps0_lt_omega e : e <ε₀ ω^e.
-  Proof. apply eps0_lt_exp_S. Qed.
+  Fact eps0_add_below_omega : ∀ e f g, e <ε₀ ω^g → f <ε₀ ω^g → e +₀ f <ε₀ ω^g.
+  Proof. intros [[] ] [[] ] []; apply E0_add_below_omega. Qed.
 
-  Hint Resolve eps0_lt_omega : core.
+  (* A "tail form" is a +₀ ω^e but it is not unique unless a is chosen
+     the least possible for this value, see eps0_least_split *)
 
-  Fact eps0_omega_mono_lt : ∀ e f, e <ε₀ f → ω^e <ε₀ ω^f.
-  Proof. intros [] [] ?; constructor; constructor 2; left; auto. Qed.
-
-  Fact eps0_omega_mono_le e f : e ≤ε₀ f → ω^e ≤ε₀ ω^f.
-  Proof. intros [ | <- ]; auto; left; now apply eps0_omega_mono_lt. Qed.
-
-  Fact eps0_omega_inj e f : ω^e = ω^f → e = f.
+  Fact eps0_tf_fun_right : ∀ a b e f, a +₀ ω^e = b +₀ ω^f → e = f.
   Proof.
-    intros E.
-    destruct (eps0_lt_sdec e f) as [ e f H | | e f H ]; auto;
-      apply eps0_omega_mono_lt in H; rewrite E in H; now apply eps0_lt_irrefl in H.
+    intros [] [] [] []; rewrite !eps0_eq_iff; simpl.
+    apply E0_add_omega_fun_right.
   Qed.
-  
-  Fact eps0_add_exp_S_omega e i : ω^⟨e,i⟩ +₀ ω^e = ω^⟨e,i +ₚ 1ₚ⟩.
-  Proof. unfold eps0_omega; rewrite eps0_add_exp_S; auto. Qed.
 
-  Fact eps0_one_eq_omega e : 1₀ = ω^e → e = 0₀.
+  (** A "head normal form" is ω^⟨e,i⟩ +₀ f with f <ε₀ ω^e 
+      and it is unique (for non-zero ordinals) *)
+
+  Fact eps0_eq_hnf_inv : ∀ e₁ i₁ f₁ e₂ i₂ f₂,
+      ω^⟨e₁,i₁⟩ +₀ f₁ = ω^⟨e₂,i₂⟩ +₀ f₂
+    → f₁ <ε₀ ω^e₁
+    → f₂ <ε₀ ω^e₂
+    → e₁ = e₂ ∧ i₁ = i₂ ∧ f₁ = f₂.
   Proof.
-    rewrite <- eps0_omega_zero.
-    now intros <-%eps0_omega_inj.
+    intros (e & He) i ([l] & Hl) (f & Hf) j ([m] & Hm)
+           E%eps0_eq_iff H1 H2.
+    rewrite !eps0_eq_iff; simpl in *.
+    rewrite !E0_add_head_normal in E; auto.
+    now inversion E.
   Qed.
 
-  Fact eps0_zero_lt_omega e : 0₀ <ε₀ ω^e.
-  Proof. apply eps0_lt_zero_exp_S. Qed.
-
-  Hint Resolve eps0_zero_lt_omega : core.
-
-  Fact eps0_zero_neq_omega e : 0₀ ≠ ω^e.
-  Proof. 
-    intros H.
-    apply (@eps0_lt_irrefl 0₀).
-    rewrite H at 2.
-    apply eps0_zero_lt_omega.
-  Qed.
-
-  Fact eps0_add_below_omega e f g : e <ε₀ ω^g → f <ε₀ ω^g → e +₀ f <ε₀ ω^g.
-  Proof. revert e f g; intros [[] ] [[] ] []; apply E0_add_below_omega. Qed.
-
-  Fact eps0_lt_head_split_inv e₁ i₁ f₁ e₂ i₂ f₂ :
+  Fact eps0_lt_hnf_inv : ∀ e₁ i₁ f₁ e₂ i₂ f₂,
       f₁ <ε₀ ω^e₁
     → f₂ <ε₀ ω^e₂
     → ω^⟨e₁,i₁⟩ +₀ f₁ <ε₀ ω^⟨e₂,i₂⟩ +₀ f₂
     ↔ e₁ <ε₀ e₂ ∨ e₁ = e₂ ∧ (i₁ < i₂ ∨ i₁ = i₂ ∧ f₁ <ε₀ f₂).
   Proof.
-    rewrite !eps0_eq_iff.
-    revert e₁ i₁ f₁ e₂ i₂ f₂.
-    intros (e & He) i ([l] & Hl) (f & Hf) j ([m] & Hm) H1 H2; simpl in *.
+    intros (e & He) i ([l] & Hl) (f & Hf) j ([m] & Hm) H1 H2;
+    rewrite eps0_eq_iff in *; simpl in *.
     rewrite !E0_add_head_normal in *; auto.
     split; intros H3.
     + apply E0_lt_inv, lex_list_cons_inv in H3
@@ -592,90 +591,7 @@ Section eps0_omega.
       * now constructor 3.
   Qed.
 
-  Fact eps0_lt_head_split_inv_left e₁ i₁ e₂ i₂ f₂ :
-      f₂ <ε₀ ω^e₂
-    → ω^⟨e₁,i₁⟩ <ε₀ ω^⟨e₂,i₂⟩ +₀ f₂
-    ↔ e₁ <ε₀ e₂ ∨ e₁ = e₂ ∧ (i₁ < i₂ ∨ i₁ = i₂ ∧ 0₀ <ε₀ f₂).
-  Proof.
-    intro.
-    rewrite <- (eps0_add_zero_right ω^⟨e₁,_⟩), eps0_lt_head_split_inv; auto.
-    firstorder.
-  Qed.
-
-  Fact eps0_lt_head_split_inv_right e₁ i₁ f₁ e₂ i₂ :
-      f₁ <ε₀ ω^e₁
-    → ω^⟨e₁,i₁⟩ +₀ f₁ <ε₀ ω^⟨e₂,i₂⟩
-    ↔ e₁ <ε₀ e₂ ∨ e₁ = e₂ ∧ i₁ < i₂.
-  Proof.
-    intro.
-    rewrite <- (eps0_add_zero_right ω^⟨e₂,_⟩), eps0_lt_head_split_inv; auto.
-    apply or_iff_compat_l, and_iff_compat_l.
-    split; auto.
-    intros [ | (_ & ?%eps0_zero_not_gt) ]; now auto.
-  Qed.
-
-  Fact eps0_lt_head_split_inv_both e₁ i₁ e₂ i₂ :
-      ω^⟨e₁,i₁⟩ <ε₀ ω^⟨e₂,i₂⟩
-    ↔ e₁ <ε₀ e₂ ∨ e₁ = e₂ ∧ i₁ < i₂.
-  Proof.
-    rewrite <- (eps0_add_zero_right ω^⟨e₁,_⟩).
-    apply eps0_lt_head_split_inv_right; auto.
-  Qed.
-
-  Fact eps0_lt_zero_head e i f : 0₀ <ε₀ ω^⟨e,i⟩ +₀ f.
-  Proof. apply eps0_lt_le_trans with ω^⟨e,i⟩; auto. Qed.
-
-  Hint Resolve eps0_lt_zero_head : core.
-
-  Fact eps0_not_head_split_lt_zero e i f : ¬ ω^⟨e,i⟩ +₀ f <ε₀ 0₀.
-  Proof. apply eps0_zero_not_gt. Qed.
-
-  Fact eps0_not_eps_S_lt_zero e i : ¬ ω^⟨e,i⟩ <ε₀ 0₀.
-  Proof. apply eps0_zero_not_gt. Qed.
-
-  Fact eps0_head_split_uniq e₁ i₁ f₁ e₂ i₂ f₂ :
-      ω^⟨e₁,i₁⟩ +₀ f₁ = ω^⟨e₂,i₂⟩ +₀ f₂
-    → f₁ <ε₀ ω^e₁
-    → f₂ <ε₀ ω^e₂
-    → e₁ = e₂ ∧ i₁ = i₂ ∧ f₁ = f₂.
-  Proof.
-    revert e₁ i₁ f₁ e₂ i₂ f₂.
-    intros (e & He) i ([l] & Hl) (f & Hf) j ([m] & Hm)
-           E%eps0_eq_iff H1 H2.
-    rewrite !eps0_eq_iff; simpl in *.
-    rewrite !E0_add_head_normal in E; auto.
-    now inversion E.
-  Qed.
-
-  Fact eps0_head_split_uniq' e₁ i₁ e₂ i₂ f₂ :
-      ω^⟨e₁,i₁⟩ = ω^⟨e₂,i₂⟩ +₀ f₂
-    → f₂ <ε₀ ω^e₂
-    → e₁ = e₂ ∧ i₁ = i₂ ∧ f₂ = 0₀.
-  Proof.
-    rewrite <- (eps0_add_zero_right ω^⟨e₁,i₁⟩).
-    intros H1 H2; revert H1.
-    intros (-> & -> & <-)%eps0_head_split_uniq; auto.
-  Qed.
-
-  Fact eps0_eps_S_uniq e₁ i₁ e₂ i₂ :
-    ω^⟨e₁,i₁⟩ = ω^⟨e₂,i₂⟩ → e₁ = e₂ ∧ i₁ = i₂.
-  Proof.
-     rewrite <- (eps0_add_zero_right ω^⟨_,i₁⟩),
-             <- (eps0_add_zero_right ω^⟨_,i₂⟩).
-     intros (-> & -> & _)%eps0_head_split_uniq; auto.
-  Qed.
-
-  Fact eps0_zero_neq_head e i f : 0₀ ≠ ω^⟨e,i⟩ +₀ f.
-  Proof.
-    intros E.
-    apply (@eps0_lt_irrefl 0₀).
-    rewrite E at 2.
-    apply eps0_lt_le_trans with (1 := eps0_lt_zero_exp_S e i).
-    rewrite <- (eps0_add_zero_right ω^⟨_,i⟩) at 1.
-    apply eps0_add_mono; auto.
-  Qed.
-
-  Fact eps0_add_head_lt e₁ i₁ f₁ e₂ i₂ f₂ :
+  Fact eps0_add_hnf_lt e₁ i₁ f₁ e₂ i₂ f₂ :
       e₁ <ε₀ e₂
     → f₁ <ε₀ ω^e₁
     → f₂ <ε₀ ω^e₂
@@ -688,25 +604,7 @@ Section eps0_omega.
     rewrite E0_add_head_lt; auto.
   Qed.
 
-  Fact eps0_add_head_lt' e₁ i₁ e₂ i₂ f₂ :
-      e₁ <ε₀ e₂
-    → f₂ <ε₀ ω^e₂
-    → ω^⟨e₁,i₁⟩ +₀ (ω^⟨e₂,i₂⟩ +₀ f₂) = ω^⟨e₂,i₂⟩ +₀ f₂.
-  Proof.
-    intros H1 H2.
-    rewrite <- (eps0_add_zero_right ω^⟨e₁,i₁⟩).
-    apply eps0_add_head_lt; auto.
-  Qed.
-
-  Fact eps0_add_head_lt'' e₁ i₁ e₂ i₂ :
-      e₁ <ε₀ e₂ → ω^⟨e₁,i₁⟩ +₀ ω^⟨e₂,i₂⟩ = ω^⟨e₂,i₂⟩.
-  Proof.
-    intros H.
-    rewrite <- (eps0_add_zero_right ω^⟨_,i₂⟩).
-    apply eps0_add_head_lt'; auto.
-  Qed.
-
-  Fact eps0_add_head_eq e i₁ f₁ i₂ f₂ :
+  Fact eps0_add_hnf_eq e i₁ f₁ i₂ f₂ :
       f₁ <ε₀ ω^e
     → f₂ <ε₀ ω^e
     → (ω^⟨e,i₁⟩ +₀ f₁) +₀ (ω^⟨e,i₂⟩ +₀ f₂) = ω^⟨e,i₁ +ₚ i₂⟩ +₀ f₂.
@@ -718,16 +616,7 @@ Section eps0_omega.
     rewrite E0_add_head_eq; auto.
   Qed.
 
-  Fact eps0_add_head_eq' e i₁ i₂ f₂ :
-      f₂ <ε₀ ω^e
-    → ω^⟨e,i₁⟩ +₀ (ω^⟨e,i₂⟩ +₀ f₂) = ω^⟨e,i₁ +ₚ i₂⟩ +₀ f₂.
-  Proof.
-    intros.
-    rewrite <- (eps0_add_zero_right ω^⟨e,i₁⟩).
-    rewrite eps0_add_head_eq; auto.
-  Qed.
-
-  Fact eps0_add_head_gt e₁ i₁ f₁ e₂ i₂ f₂ :
+  Fact eps0_add_hnf_gt e₁ i₁ f₁ e₂ i₂ f₂ :
       e₂ <ε₀ e₁
     → f₁ <ε₀ ω^e₁
     → f₂ <ε₀ ω^e₂
@@ -741,13 +630,13 @@ Section eps0_omega.
     apply E0_add_head_gt; auto.
   Qed.
 
-  Section eps0_head_rect.
+  Section eps0_hnf_rect.
 
     Variables (P : ε₀ → Type)
               (HP0 : P 0₀)
               (HP1 : ∀ e i f, f <ε₀ ω^e → P e → P f → P (ω^⟨e,i⟩ +₀ f)).
 
-    Theorem eps0_head_rect : ∀e, P e.
+    Theorem eps0_hnf_rect : ∀e, P e.
     Proof.
       intros (e & he); revert e he.
       apply cnf_head_rect.
@@ -756,876 +645,235 @@ Section eps0_omega.
         refine (@eps0_pirr P _ _ _ _ _ (@HP1 _ i _ _ He Hf)); auto.
     Qed.
 
-  End eps0_head_rect.
+  End eps0_hnf_rect.
 
-  Lemma eps0_lt_exp_S_inv a e n :
+  (**********************)
+
+  Fact eps0_lt_omega e : e <ε₀ ω^e.
+  Proof. apply eps0_lt_exp. Qed.
+
+  Hint Resolve eps0_lt_omega : core.
+
+  Fact eps0_omega_mono_lt : ∀ e f, e <ε₀ f → ω^e <ε₀ ω^f.
+  Proof. unfold eps0_omega; auto. Qed.
+
+  Fact eps0_omega_mono_le e f : e ≤ε₀ f → ω^e ≤ε₀ ω^f.
+  Proof. intros [ | <- ]; auto; left; now apply eps0_omega_mono_lt. Qed.
+
+  Fact eps0_omega_inj e f : ω^e = ω^f → e = f.
+  Proof. now intros []%eps0_exp_inj. Qed.
+
+  Fact eps0_add_exp_omega e i : ω^⟨e,i⟩ +₀ ω^e = ω^⟨e,i +ₚ 1ₚ⟩.
+  Proof. unfold eps0_omega; rewrite eps0_add_exp; auto. Qed.
+
+  Fact eps0_one_eq_omega e : 1₀ = ω^e → e = 0₀.
+  Proof. rewrite <- eps0_omega_zero; now intros <-%eps0_omega_inj. Qed.
+
+  Fact eps0_zero_lt_omega e : 0₀ <ε₀ ω^e.
+  Proof. apply eps0_lt_zero_exp. Qed.
+
+  Hint Resolve eps0_zero_lt_omega : core.
+
+  Fact eps0_zero_neq_omega e : 0₀ ≠ ω^e.
+  Proof. apply eps0_zero_neq_exp. Qed.
+
+  (** head_normal_forms *)
+
+  Fact eps0_lt_exp_hnf_inv e₁ i₁ e₂ i₂ f₂ :
+      f₂ <ε₀ ω^e₂
+    → ω^⟨e₁,i₁⟩ <ε₀ ω^⟨e₂,i₂⟩ +₀ f₂
+    ↔ e₁ <ε₀ e₂ ∨ e₁ = e₂ ∧ (i₁ < i₂ ∨ i₁ = i₂ ∧ 0₀ <ε₀ f₂).
+  Proof.
+    intro.
+    rewrite <- (eps0_add_zero_right ω^⟨e₁,_⟩),
+                eps0_lt_hnf_inv; auto.
+    firstorder.
+  Qed.
+
+  Fact eps0_lt_hnf_exp_inv e₁ i₁ f₁ e₂ i₂ :
+      f₁ <ε₀ ω^e₁
+    → ω^⟨e₁,i₁⟩ +₀ f₁ <ε₀ ω^⟨e₂,i₂⟩
+    ↔ e₁ <ε₀ e₂ ∨ e₁ = e₂ ∧ i₁ < i₂.
+  Proof.
+    intro.
+    rewrite <- (eps0_add_zero_right ω^⟨e₂,_⟩),
+                eps0_lt_hnf_inv; auto.
+    apply or_iff_compat_l, and_iff_compat_l.
+    split; auto.
+    intros [ | (_ & ?%eps0_zero_not_gt) ]; now auto.
+  Qed.
+
+  Fact eps0_lt_exp_inv e₁ i₁ e₂ i₂ :
+      ω^⟨e₁,i₁⟩ <ε₀ ω^⟨e₂,i₂⟩
+    ↔ e₁ <ε₀ e₂ ∨ e₁ = e₂ ∧ i₁ < i₂.
+  Proof.
+    rewrite <- (eps0_add_zero_right ω^⟨e₁,_⟩).
+    apply eps0_lt_hnf_exp_inv; auto.
+  Qed.
+
+  Fact eps0_lt_zero_hnf e i f : 0₀ <ε₀ ω^⟨e,i⟩ +₀ f.
+  Proof. apply eps0_lt_le_trans with ω^⟨e,i⟩; auto. Qed.
+
+  Hint Resolve eps0_lt_zero_hnf : core.
+
+(*
+  Fact eps0_not_head_split_lt_zero e i f : ¬ ω^⟨e,i⟩ +₀ f <ε₀ 0₀.
+  Proof. apply eps0_zero_not_gt. Qed.
+
+  Fact eps0_not_eps_S_lt_zero e i : ¬ ω^⟨e,i⟩ <ε₀ 0₀.
+  Proof. apply eps0_zero_not_gt. Qed.
+*)
+
+  Fact eps0_eq_exp_hnf_inv e₁ i₁ e₂ i₂ f₂ :
+      ω^⟨e₁,i₁⟩ = ω^⟨e₂,i₂⟩ +₀ f₂
+    → f₂ <ε₀ ω^e₂
+    → e₁ = e₂ ∧ i₁ = i₂ ∧ f₂ = 0₀.
+  Proof.
+    rewrite <- (eps0_add_zero_right ω^⟨e₁,i₁⟩).
+    intros H1 H2; revert H1.
+    intros (-> & -> & <-)%eps0_eq_hnf_inv; auto.
+  Qed.
+
+  Fact eps0_zero_neq_hnf e i f : 0₀ ≠ ω^⟨e,i⟩ +₀ f.
+  Proof. intro E; apply (@eps0_lt_irrefl 0₀); rewrite E at 2; auto. Qed.
+
+  Fact eps0_add_exp_hnf_lt e₁ i₁ e₂ i₂ f₂ :
+      e₁ <ε₀ e₂
+    → f₂ <ε₀ ω^e₂
+    → ω^⟨e₁,i₁⟩ +₀ (ω^⟨e₂,i₂⟩ +₀ f₂) = ω^⟨e₂,i₂⟩ +₀ f₂.
+  Proof.
+    intros H1 H2.
+    rewrite <- (eps0_add_zero_right ω^⟨e₁,i₁⟩).
+    apply eps0_add_hnf_lt; auto.
+  Qed.
+
+  Fact eps0_add_exp_lt e₁ i₁ e₂ i₂ :
+      e₁ <ε₀ e₂ → ω^⟨e₁,i₁⟩ +₀ ω^⟨e₂,i₂⟩ = ω^⟨e₂,i₂⟩.
+  Proof.
+    intro.
+    rewrite <- (eps0_add_zero_right ω^⟨_,i₂⟩).
+    apply eps0_add_exp_hnf_lt; auto.
+  Qed.
+
+  Fact eps0_add_exp_hnf_eq e i₁ i₂ f₂ :
+      f₂ <ε₀ ω^e
+    → ω^⟨e,i₁⟩ +₀ (ω^⟨e,i₂⟩ +₀ f₂) = ω^⟨e,i₁ +ₚ i₂⟩ +₀ f₂.
+  Proof.
+    intro.
+    rewrite <- (eps0_add_zero_right ω^⟨e,i₁⟩).
+    rewrite eps0_add_hnf_eq; auto.
+  Qed.
+
+  (* Ordinals below ω^e.n are of the form
+        - 0
+        - ω^e.i +₀ b with i < n and b < ω^e
+        - or < ω^f.i with f <ε₀ e  *)
+
+  Lemma eps0_below_exp_inv a e n :
       a <ε₀ ω^⟨e,n⟩
     → (a = 0₀)
-    + { i : _ & { b | a = ω^⟨e,i⟩ +₀ b ∧ i < n ∧ b <ε₀ ω^e } }
-    + { f : _ & { i | a <ε₀ ω^⟨f,i⟩ ∧ f <ε₀ e } }.
+    + {i : _ & {b | a = ω^⟨e,i⟩ +₀ b ∧ i < n ∧ b <ε₀ ω^e}}
+    + {f : _ & {i | a <ε₀ ω^⟨f,i⟩ ∧ f <ε₀ e}}.
   Proof.
-    destruct a as [ | g i h H _ _ ] using eps0_head_rect.
+    destruct a as [ | g i h H _ _ ] using eps0_hnf_rect.
     + now do 2 left.
-    + intros H1.
-      destruct n as [ | n ].
+    + intros H1%eps0_lt_hnf_exp_inv; auto.
+      destruct (pos_one_or_succ n) as [ -> | (j & ->) ].
       * right.
-        exists g, (S i).
-        apply eps0_lt_head_split_inv_right in H1
-          as [ H1 | (_ & ?) ]; lia || auto.
-        split; auto.
-        apply eps0_lt_head_split_inv_right; auto.
-      * apply eps0_lt_head_split_inv_right in H1; auto.
-        destruct (eps0_le_lt_dec e g) as [ C | C ].
+        exists g, (i +ₚ 1ₚ).
+        rewrite eps0_lt_hnf_exp_inv; auto.
+        destruct H1 as [ | (-> & []%pos_not_lt_one) ]; auto.
+      * destruct (eps0_le_lt_dec e g) as [ C | C ].
         - left; right; exists i, h.
-          destruct H1 as [ H1 | (-> & H1) ]; eauto.
+          destruct H1 as [ | (-> & ?) ]; eauto.
           destruct (@eps0_lt_irrefl e); eauto.
-        - right; exists g, (S i); split; auto.
-          apply eps0_lt_head_split_inv_right; auto.
+        - right; exists g, (i +ₚ 1ₚ); split; auto.
+          rewrite eps0_lt_hnf_exp_inv; auto.
   Qed.
 
   (** inversion for _ <ε₀ ω^_ *)
-  Lemma eps0_lt_omega_inv a e : a <ε₀ ω^e → (a = 0₀) + { f : ε₀ & { n | a <ε₀ ω^⟨f,n⟩ ∧ f <ε₀ e } }.
-  Proof. intros [[ -> | (i & ? & ? & []%pos_not_lt_one & _) ] | ]%eps0_lt_exp_S_inv; auto. Qed.
+  Lemma eps0_below_omega_inv a e :
+      a <ε₀ ω^e
+    → (a = 0₀) 
+    + {f : ε₀ & {n | a <ε₀ ω^⟨f,n⟩ ∧ f <ε₀ e}}.
+  Proof. intros [[ -> | (i & ? & ? & []%pos_not_lt_one & _) ] | ]%eps0_below_exp_inv; auto. Qed.
+
+  Fact eps0_add_lt_omega a e : a <ε₀ ω^e → a +₀ ω^e = ω^e.
+  Proof.
+    intros [ -> | (f & n & []) ]%eps0_below_omega_inv.
+    + now rewrite eps0_add_zero_left.
+    + apply eps0_le_antisym; auto.
+      apply eps0_le_trans with (ω^⟨f,n⟩ +₀ ω^e); auto.
+      unfold eps0_omega; rewrite eps0_add_exp_lt; auto.
+  Qed.
 
   (** inversion for _ < ω^(_+1) *)
-  Lemma eps0_lt_omega_succ_inv f e : f <ε₀ ω^(S₀ e) → { n | f <ε₀ ω^⟨e,n⟩ }.
+  Lemma eps0_below_omega_succ_inv f e : f <ε₀ ω^(S₀ e) → { n | f <ε₀ ω^⟨e,n⟩ }.
   Proof.
-    intros [ -> | (a & n & H1 & H2%eps0_succ_next_inv) ]%eps0_lt_omega_inv.
+    intros [ -> | (a & n & H1 & H2%eps0_succ_next_inv) ]%eps0_below_omega_inv.
     + exists 0; auto.
-    + exists n; apply eps0_lt_le_trans with (1 := H1), eps0_exp_S_mono; auto.
+    + exists n; apply eps0_lt_le_trans with (1 := H1); auto.
   Qed.
-  
+
+(*
   Hint Resolve eps0_exp_S_mono_left eps0_exp_S_mono : core.
-  
-  Fact eps0_add_exp_S_omega_le e n m : n < m → ω^⟨e,n⟩ +₀ ω^e ≤ε₀ ω^⟨e,m⟩.
+  *)
+
+  Fact eps0_le_add_exp_omega e n m : n < m → ω^⟨e,n⟩ +₀ ω^e ≤ε₀ ω^⟨e,m⟩.
   Proof.
-    intro H; unfold eps0_omega.
-    rewrite eps0_add_exp_S.
-    apply eps0_exp_S_mono; auto.
-    unfold pos_one, pos_add; lia.
+    intros H%pos_lt_iff_le_succ; unfold eps0_omega.
+    rewrite eps0_add_exp; auto.
   Qed.
   
-  Lemma eps0_add_below_exp_S b c e n : b <ε₀ ω^⟨e,n⟩ → c <ε₀ ω^e → b+₀c <ε₀ ω^⟨e,n⟩.
+  Lemma eps0_add_below_exp b c e n : b <ε₀ ω^⟨e,n⟩ → c <ε₀ ω^e → b+₀c <ε₀ ω^⟨e,n⟩.
   Proof.
-    intros [ [ -> | (u & i & -> & []) ] | (u & i & []) ]%eps0_lt_exp_S_inv [ -> | (v & j & H2 & H3) ]%eps0_lt_omega_inv.
+    intros [ [ -> | (u & i & -> & []) ] | (u & i & []) ]%eps0_below_exp_inv
+           [ -> | (v & j & H2 & H3) ]%eps0_below_omega_inv.
     + rewrite eps0_add_zero_left; auto.
     + rewrite eps0_add_zero_left; apply eps0_lt_trans with (1 := H2); auto.
     + rewrite eps0_add_zero_right.
-      apply eps0_lt_le_trans with (2 := eps0_add_exp_S_omega_le _ H); auto.
+      apply eps0_lt_le_trans with (2 := eps0_le_add_exp_omega _ H); auto.
     + rewrite eps0_add_assoc.
-      apply eps0_lt_le_trans with (2 := eps0_add_exp_S_omega_le _ H); auto.
+      apply eps0_lt_le_trans with (2 := eps0_le_add_exp_omega _ H); auto.
       apply eps0_add_mono_right, eps0_add_below_omega; auto.
-      now apply eps0_lt_trans with (1 := H2), eps0_exp_S_mono_left.
-    + rewrite eps0_add_zero_right.
-      now apply eps0_lt_trans with (1 := H), eps0_exp_S_mono_left.
+      now apply eps0_lt_trans with (1 := H2), eps0_exp_mono_left.
+    + rewrite eps0_add_zero_right; apply eps0_lt_trans with (1 := H); auto.
     + apply eps0_lt_le_trans with ω^e.
       * apply eps0_add_below_omega; auto.
-        - now apply eps0_lt_trans with (1 := H), eps0_exp_S_mono_left.
-        - now apply eps0_lt_trans with (1 := H2), eps0_exp_S_mono_left.
-      * apply eps0_exp_S_mono; auto.
-        unfold pos_one; lia.
+        - now apply eps0_lt_trans with (1 := H), eps0_exp_mono_left.
+        - now apply eps0_lt_trans with (1 := H2), eps0_exp_mono_left.
+      * apply eps0_exp_mono; auto.
   Qed.
 
-  Section eps0_head_pos_rect.
+  Section eps0_hnf_pos_rect.
 
     Variables (P : ε₀ → Type)
               (HP0 : P 0₀)
               (HP1 : ∀i, P ω^⟨0₀,i⟩) 
               (HP2 : ∀ e i f, 0₀ <ε₀ e → f <ε₀ ω^e → P e → P f → P (ω^⟨e,i⟩ +₀ f)).
 
-    Theorem eps0_head_pos_rect : ∀e, P e.
+    Theorem eps0_hnf_pos_rect : ∀e, P e.
     Proof.
-      induction e as [ | e n f H ] using eps0_head_rect; trivial.
+      induction e as [ | e n f H ] using eps0_hnf_rect; trivial.
       destruct (eps0_zero_or_pos e) as [ -> | G ].
       + assert (f = 0₀) as ->.
         1:{ rewrite eps0_omega_zero in H.
             now apply eps0_lt_one in H. }
-        rewrite eps0_add_zero_right; trivial.
+        now rewrite eps0_add_zero_right.
       + now apply HP2.
     Qed.
 
-  End eps0_head_pos_rect.
+  End eps0_hnf_pos_rect.
 
 End eps0_omega.
 
 Hint Resolve eps0_lt_omega 
-             eps0_lt_zero_exp_S
+             eps0_lt_zero_exp
              eps0_zero_lt_omega 
-             eps0_lt_zero_head : core.
+             eps0_lt_zero_hnf : core.
 
-#[global] Notation "ω^⟨ e , i ⟩" := (eps0_exp_S e i).
+#[global] Notation "ω^⟨ e , i ⟩" := (eps0_exp e i).
 #[global] Notation "ω^ e" := (eps0_omega e).
-
-Fact eps0_add_lt_omega : ∀ a e, a <ε₀ ω^e → a +₀ ω^e = ω^e.
-Proof.
-  intros a e.
-  destruct (eps0_zero_or_pos e) as [ -> | He ].
-  + intros Ha.
-    rewrite eps0_omega_zero in Ha.
-    apply eps0_lt_one in Ha as ->.
-    now rewrite eps0_add_zero_left.
-  + revert a e He.
-    intros [a Ha] [e He] He' H.
-    apply eps0_eq_iff; simpl in H |- *.
-    revert H; apply E0_add_lt_omega; auto.
-    intros ->.
-    revert He'; apply E0_lt_irrefl.
-Qed.
-
-Lemma eps0_add_omega_fun_right : ∀ a b e f, a +₀ ω^e = b +₀ ω^f → e = f.
-Proof.
-  intros [] [] [] []; rewrite !eps0_eq_iff; simpl.
-  apply E0_add_omega_fun_right.
-Qed.
-
-Section eps0_mpos.
-
-  (** pos := nat viewed as 1, 2, ... and not 0, 1, ... *)
-
-  (** The operation (θ : ε₀) (n : pos) => θ.(1+n) *)
-  Inductive eps0_mpos_gr n : ε₀ → ε₀ → Prop :=
-    | eps0_mpos_gr_0 : eps0_mpos_gr n 0₀ 0₀
-    | eps0_mpos_gr_1 α i β : β <ε₀ ω^α → eps0_mpos_gr n (ω^⟨α,i⟩ +₀ β) (ω^⟨α,i *ₚ n⟩ +₀ β).
-
-  Fact eps0_mpos_fun n e1 f1 e2 f2 : eps0_mpos_gr n e1 f1 → eps0_mpos_gr n e2 f2 → e1 = e2 → f1 = f2.
-  Proof.
-    do 2 destruct 1; auto.
-    + now intros ?%eps0_zero_neq_exp_S_add.
-    + symm; now intros ?%eps0_zero_neq_exp_S_add.
-    + intros (? & [])%eps0_head_split_uniq; subst; auto.
-  Qed.
-
-  Definition eps0_mpos_pwc e n : sig (eps0_mpos_gr n e).
-  Proof.
-    destruct e as [ | e i f H ] using eps0_head_rect.
-    + exists 0₀; constructor.
-    + exists (ω^⟨e,i *ₚ n⟩ +₀ f); now constructor.
-  Qed.
-
-  Definition eps0_mpos e n := π₁ (eps0_mpos_pwc e n).
-
-  Fact eps0_mpos_spec e n : eps0_mpos_gr n e (eps0_mpos e n).
-  Proof. apply (proj2_sig _). Qed.
-
-  Fact eps0_mpos_fix_0 n : eps0_mpos 0₀ n = 0₀.
-  Proof. apply eps0_mpos_fun with (1 := eps0_mpos_spec _ _) (3 := eq_refl); constructor. Qed.
-
-  Fact eps0_mpos_fix_1 n α i β : β <ε₀ ω^α → eps0_mpos (ω^⟨α,i⟩ +₀ β) n = ω^⟨α,i *ₚ n⟩ +₀ β.
-  Proof. intros; apply eps0_mpos_fun with (1 := eps0_mpos_spec _ _) (3 := eq_refl); now constructor. Qed.
-
-  Fact eps0_mpos_exp_S n α i : eps0_mpos ω^⟨α,i⟩ n = ω^⟨α,i *ₚ n⟩.
-  Proof. 
-    rewrite <- (eps0_add_zero_right ω^⟨_,i⟩), eps0_mpos_fix_1; auto.
-    now rewrite eps0_add_zero_right.
-  Qed.
-
-  Fact eps0_mpos_O e : eps0_mpos e 1ₚ = e.
-  Proof.
-    destruct e using eps0_head_rect.
-    + now rewrite eps0_mpos_fix_0.
-    + rewrite eps0_mpos_fix_1, pos_mul_one_right; auto.
-  Qed.
-
-  Fact eps0_mpos_omega_add n α β : β <ε₀ ω^α → eps0_mpos (ω^α +₀ β) n = ω^⟨α,n⟩ +₀ β.
-  Proof.
-    intros; unfold eps0_omega.
-    rewrite eps0_mpos_fix_1; auto.
-  Qed.
-
-  Fact eps0_mpos_omega n α : eps0_mpos ω^α n = ω^⟨α,n⟩.
-  Proof.
-    rewrite <- (eps0_add_zero_right ω^α), eps0_mpos_omega_add; auto.
-    now rewrite eps0_add_zero_right.
-  Qed.
-
-  Fact eps0_mpos_plus e i j : eps0_mpos e i +₀ eps0_mpos e j = eps0_mpos e (i +ₚ j).
-  Proof.
-    destruct e using eps0_head_rect.
-    + now rewrite !eps0_mpos_fix_0, eps0_add_zero_left.
-    + rewrite !eps0_mpos_fix_1; auto.
-      rewrite eps0_add_head_eq, pos_mul_distr_right; auto.
-  Qed.
-
-  Fact eps0_mpos_mult e i j : eps0_mpos (eps0_mpos e i) j = eps0_mpos e (i *ₚ j).
-  Proof.
-    destruct e using eps0_head_rect.
-    + now rewrite !eps0_mpos_fix_0.
-    + rewrite !eps0_mpos_fix_1, pos_mul_assoc; auto.
-  Qed.
-
-  Fact eps0_mpos_mono_left a b m n : a <ε₀ b → m ≤ n → eps0_mpos a m <ε₀ eps0_mpos b n.
-  Proof.
-    intros Hab Hmn.
-    destruct a as [ | e i f H1 _ _ ] using eps0_head_rect;
-      destruct b as [ | g j h H2 _ _ ] using eps0_head_rect.
-    + now apply eps0_lt_irrefl in Hab.
-    + rewrite eps0_mpos_fix_0, eps0_mpos_fix_1; auto.
-    + now apply eps0_not_head_split_lt_zero in Hab.
-    + apply eps0_lt_head_split_inv in Hab; auto.
-      rewrite !eps0_mpos_fix_1; auto.
-      apply eps0_lt_head_split_inv; auto.
-      destruct Hab as [ | (<- & [ | (<- & ?) ]) ]; auto.
-      * right; split; auto; left.
-        now apply pos_mul_mono_left.
-      * apply pos_le_lt_iff in Hmn as [ -> | Hmn ]; auto.
-        right; split; auto; left.
-        now apply pos_mul_mono_right.
-  Qed.
-
-  Fact eps0_mpos_gt_zero a n : 0₀ <ε₀ a → 0₀ <ε₀ eps0_mpos a n.
-  Proof.
-    intros H.
-    apply eps0_mpos_mono_left with (n := n) (m := n) in H; auto.
-    now rewrite eps0_mpos_fix_0 in H.
-  Qed.
-
-  Hint Resolve eps0_mpos_mono_left eps0_mpos_gt_zero : core.
-
-  Fact eps0_mpos_mono_right a n m : 0₀ <ε₀ a → n < m → eps0_mpos a n <ε₀ eps0_mpos a m.
-  Proof.
-    intros H1 H2.
-    destruct a as [ | e i f H _ _ ] using eps0_head_rect.
-    + now apply eps0_lt_irrefl in H1.
-    + rewrite !eps0_mpos_fix_1; auto.
-      apply eps0_lt_head_split_inv; auto.
-      right; split; auto; left.
-      now apply pos_mul_mono_right.
-  Qed.
-
-  Fact eps0_mpos_mono_right_le a n m : n ≤ m → eps0_mpos a n ≤ε₀ eps0_mpos a m.
-  Proof.
-    destruct (eq_nat_dec n m) as [ <- | ]; auto; intro.
-    destruct (eps0_zero_or_pos a) as [ -> | ].
-    + rewrite !eps0_mpos_fix_0; auto.
-    + left; apply eps0_mpos_mono_right; auto; lia.
-  Qed.
-
-  Fact eps0_mpos_mono a b m n : a ≤ε₀ b → m ≤ n → eps0_mpos a m ≤ε₀ eps0_mpos b n.
-  Proof.
-    intros [ H1 | -> ].
-    + left; now apply eps0_mpos_mono_left.
-    + apply eps0_mpos_mono_right_le.
-  Qed.
-
-  Fact eps0_mpos_below_omega a n e : a <ε₀ ω^e → eps0_mpos a n <ε₀ ω^e.
-  Proof.
-    intros [ -> | (f & i & H1 & H2) ] %eps0_lt_omega_inv.
-    + rewrite eps0_mpos_fix_0; auto.
-    + apply eps0_mpos_mono_left with (n := n) (m := n) in H1; auto.
-      apply eps0_lt_trans with (1 := H1).
-      rewrite eps0_mpos_exp_S.
-      apply eps0_lt_head_split_inv_both; auto.
-  Qed.
-
-  Fact eps0_mpos_below_omega' a n e i : a <ε₀ ω^⟨e,i⟩ → eps0_mpos a n <ε₀ ω^(S₀ e).
-  Proof.
-    intros H.
-    apply eps0_mpos_below_omega,
-          eps0_lt_trans with (1 := H),
-          eps0_exp_S_mono_left; auto.
-  Qed.
-
-End eps0_mpos.
-
-#[local] Hint Resolve eps0_mpos_mono_left eps0_mpos_gt_zero : core.
-
-Section eps0_momega.
-
-  (** now the operation (θ α : ε₀) => θ.ω^α *)
-  Inductive eps0_momega_gr α : ε₀ → ε₀ → Prop :=
-    | eps0_momega_gr_0 : eps0_momega_gr α 0₀ 0₀
-    | eps0_momega_gr_1 γ n β : β <ε₀ ω^γ → eps0_momega_gr α (ω^⟨γ,n⟩ +₀ β) ω^(γ+₀α).
-
-  Fact eps0_momega_fun a e1 f1 e2 f2 : eps0_momega_gr a e1 f1 → eps0_momega_gr a e2 f2 → e1 = e2 → f1 = f2.
-  Proof.
-    do 2 destruct 1; auto.
-    + now intros ?%eps0_zero_neq_exp_S_add.
-    + symm; now intros ?%eps0_zero_neq_exp_S_add.
-    + intros (? & [])%eps0_head_split_uniq; subst; auto.
-  Qed.
-
-  Definition eps0_momega_pwc e α : sig (eps0_momega_gr α e).
-  Proof.
-    destruct e as [ | e ] using eps0_head_rect.
-    + exists 0₀; constructor.
-    + exists ω^(e+₀α); now constructor.
-  Qed.
-
-  Definition eps0_momega e α := π₁ (eps0_momega_pwc e α).
-
-  Fact eps0_momega_spec e α : eps0_momega_gr α e (eps0_momega e α).
-  Proof. apply (proj2_sig _). Qed.
-
-  Fact eps0_momega_fix_0 α : eps0_momega 0₀ α = 0₀.
-  Proof. apply eps0_momega_fun with (1 := eps0_momega_spec _ _) (3 := eq_refl); constructor. Qed.
-
-  Fact eps0_momega_fix_1 γ n β α : β <ε₀ ω^γ → eps0_momega (ω^⟨γ,n⟩ +₀ β) α = ω^(γ+₀α).
-  Proof. intros; apply eps0_momega_fun with (1 := eps0_momega_spec _ _) (3 := eq_refl); now constructor. Qed.
-
-  Fact eps0_momega_exp_S γ n α : eps0_momega ω^⟨γ,n⟩ α = ω^(γ+₀α).
-  Proof. rewrite <- (eps0_add_zero_right ω^⟨_,_⟩), eps0_momega_fix_1; auto. Qed.
-
-  Fact eps0_momega_mpos a i e :
-      0₀ <ε₀ e → eps0_momega (eps0_mpos a i) e = eps0_momega a e.
-  Proof.
-    intros He.
-    destruct a using eps0_head_rect.
-    + now rewrite eps0_mpos_fix_0.
-    + rewrite eps0_mpos_fix_1; auto.
-      rewrite !eps0_momega_fix_1; auto.
-  Qed.
-
-  Fact eps0_add_mpos_momega n k e f :
-      0₀ <ε₀ f
-    → eps0_mpos e n +₀ eps0_mpos (eps0_momega e f) k
-    = eps0_mpos (eps0_momega e f) k.
-  Proof.
-    intros Hf.
-    destruct e using eps0_head_rect.
-    + now rewrite !eps0_mpos_fix_0, eps0_add_zero_left.
-    + rewrite !eps0_mpos_fix_1; auto.
-      rewrite eps0_momega_fix_1; auto.
-      rewrite !eps0_mpos_omega.
-      rewrite <- (eps0_add_zero_right ω^⟨_,k⟩).
-      rewrite eps0_add_head_lt; auto.
-  Qed.
-
-  Fact eps0_mpos_add_momega a e f i j :
-      e <ε₀ f
-    → eps0_mpos (eps0_momega a e) i +₀ eps0_mpos (eps0_momega a f) j
-    = eps0_mpos (eps0_momega a f) j.
-  Proof.
-    intros Hef.
-    destruct a using eps0_head_rect.
-    + now rewrite !eps0_momega_fix_0, !eps0_mpos_fix_0, eps0_add_zero_left.
-    + rewrite !eps0_momega_fix_1; auto.
-      rewrite !eps0_mpos_omega, eps0_add_head_lt''; auto.
-  Qed.
-
-  Fact eps0_momega_mono_left a b c :
-      a ≤ε₀ b
-    → eps0_momega a c ≤ε₀ eps0_momega b c.
-  Proof.
-    intros [ Hab | <- ]; auto.
-    destruct a as [ | e i f H1 _ _ ] using eps0_head_rect;
-      destruct b as [ | g j h H2 _ _ ] using eps0_head_rect.
-    + now apply eps0_lt_irrefl in Hab.
-    + rewrite eps0_momega_fix_0, eps0_momega_fix_1; auto.
-    + now apply eps0_zero_not_gt in Hab.
-    + rewrite !eps0_momega_fix_1; auto.
-      apply eps0_lt_head_split_inv in Hab; auto.
-      apply eps0_omega_mono_le.
-      destruct Hab as [ | (<- & _) ]; auto.
-  Qed.
-
-  Fact eps0_momega_mono_right a b c :
-      0₀ <ε₀ a
-    → b <ε₀ c 
-    → eps0_momega a b <ε₀ eps0_momega a c.
-  Proof.
-    intros H ?.
-    destruct a using eps0_head_rect.
-    + now apply eps0_lt_irrefl in H.
-    + rewrite !eps0_momega_fix_1; auto.
-      apply eps0_omega_mono_lt; auto.
-  Qed.
-
-  Fact eps0_momega_lt_pos a e :
-      0₀ <ε₀ a
-    → 0₀ <ε₀ e
-    → ω^e ≤ε₀ eps0_momega a e.
-  Proof.
-    intros Ha He.
-    destruct a using eps0_head_rect.
-    + now apply eps0_lt_irrefl in Ha.
-    + rewrite eps0_momega_fix_1; auto.
-      apply eps0_omega_mono_le; auto.
-  Qed.
-
-  Fact eps0_lt_mpos_momega a n f :
-      0₀ <ε₀ a
-    → 0₀ <ε₀ f
-    → eps0_mpos a n <ε₀ eps0_momega a f.
-  Proof.
-    intros Ha Hf.
-    destruct a using eps0_head_rect.
-    + now apply eps0_lt_irrefl in Ha.
-    + rewrite eps0_mpos_fix_1, eps0_momega_fix_1; auto.
-      apply eps0_lt_head_split_inv_right; auto.
-  Qed.
-
-  Fact eps0_momega_below_omega a b e f :
-      a <ε₀ ω^e
-    → b <ε₀ f
-    → eps0_momega a b <ε₀ ω^(e +₀ f).
-  Proof.
-    intros [ -> | (g & i & H1 & H2) ]%eps0_lt_omega_inv Hb.
-    + rewrite eps0_momega_fix_0; auto.
-    + apply eps0_le_lt_trans with (eps0_momega ω^⟨g,i⟩ b).
-      * apply eps0_momega_mono_left; auto.
-      * rewrite eps0_momega_exp_S.
-        apply eps0_omega_mono_lt.
-        apply eps0_lt_le_trans with (g +₀ f); auto.
-  Qed.
-
-  Fact eps0_momega_below_exp_S a b e n f :
-      a <ε₀ ω^⟨e,n⟩
-    → b <ε₀ f
-    → eps0_momega a b <ε₀ ω^(e +₀ f).
-  Proof.
-    intros [ [ -> | (i & c & -> & ? & ?) ] | (g & i & H1 & ?) ]%eps0_lt_exp_S_inv ?.
-    + rewrite eps0_momega_fix_0; auto.
-    + rewrite eps0_momega_fix_1; auto.
-      apply eps0_omega_mono_lt; auto.
-    + apply eps0_lt_le_weak, eps0_momega_mono_left with (c := b) in H1.
-      apply eps0_le_lt_trans with (1 := H1).
-      rewrite eps0_momega_exp_S; auto.
-      apply eps0_omega_mono_lt.
-      apply eps0_le_lt_trans with (e +₀ b); auto.
-  Qed.
-
-End eps0_momega.
-
-Section eps0_mult.
-
-  (* now the operation (γ α : ε₀) => γ.α *)
-  Inductive eps0_mult_gr γ : ε₀ → ε₀ → Prop :=
-    | eps0_mult_gr_0         : eps0_mult_gr γ 0₀ 0₀ 
-    | eps0_mult_gr_1 n       : eps0_mult_gr γ ω^⟨0₀,n⟩ (eps0_mpos γ n)
-    | eps0_mult_gr_2 α n β r : 0₀ <ε₀ α
-                             → β <ε₀ ω^α
-                             → eps0_mult_gr γ β r
-                             → eps0_mult_gr γ (ω^⟨α,n⟩ +₀ β) (eps0_mpos (eps0_momega γ α) n +₀ r).
-
-  Fact eps0_mult_fun a e1 f1 e2 f2 :
-      eps0_mult_gr a e1 f1
-    → eps0_mult_gr a e2 f2
-    → e1 = e2
-    → f1 = f2.
-  Proof.
-    intros H1; revert H1 e2 f2.
-    induction 1 as [ | n1 | e1 n1 f1 r1 H1 G1 F1 IH1 ];
-      induction 1 as [ | n2 | e2 n2 f2 r2 H2 G2 F2 _ ]; auto.
-    + now intros ?%eps0_zero_neq_exp_S.
-    + now intros ?%eps0_zero_neq_exp_S_add.
-    + symm; now intros ?%eps0_zero_neq_exp_S.
-    + now intros (_ & ->)%eps0_eps_S_uniq.
-    + intros (<- & -> & ->)%eps0_head_split_uniq'; auto.
-      contradict H2; apply eps0_lt_irrefl.
-    + symm; now intros ?%eps0_zero_neq_head.
-    + symm; intros (<- & -> & ->)%eps0_head_split_uniq'; auto.
-      contradict H1; apply eps0_lt_irrefl.
-    + intros (<- & <- & <-)%eps0_head_split_uniq; auto.
-      f_equal; eauto.
-  Qed.
-
-  Definition eps0_mult_pwc γ e : sig (eps0_mult_gr γ e).
-  Proof.
-    induction e as [ | n | e n f He Hf _ (r & Hr) ] using eps0_head_pos_rect.
-    + exists 0₀; constructor.
-    + exists (eps0_mpos γ n); constructor.
-    + exists (eps0_mpos (eps0_momega γ e) n +₀ r).
-      now constructor.
-  Qed.
-
-  Definition eps0_mult e f := π₁ (eps0_mult_pwc e f).
-
-  Infix "*₀" := eps0_mult.
-
-  Fact eps0_mult_spec e f : eps0_mult_gr e f (e *₀ f).
-  Proof. apply (proj2_sig _). Qed.
-
-  Fact eps0_mult_zero_right a : a *₀ 0₀ = 0₀.
-  Proof. apply eps0_mult_fun with (1 := eps0_mult_spec _ _) (3 := eq_refl); now constructor. Qed.
-
-  Fact eps0_mult_pos_right a n : a *₀ ω^⟨0₀,n⟩ = eps0_mpos a n.
-  Proof. apply eps0_mult_fun with (1 := eps0_mult_spec _ _) (3 := eq_refl); now constructor. Qed.
-
-  Corollary eps0_mpos_eq a n : eps0_mpos a n = a *₀ ω^⟨0₀,n⟩.
-  Proof. now rewrite eps0_mult_pos_right. Qed.
-
-  Fact eps0_mult_head_right a e n f :
-      0₀ <ε₀ e
-    → f <ε₀ ω^e
-    → a *₀ (ω^⟨e,n⟩ +₀ f)
-    = eps0_mpos (eps0_momega a e) n +₀ a *₀ f.
-  Proof.
-    intros.
-    apply eps0_mult_fun with (1 := eps0_mult_spec _ _) (3 := eq_refl); constructor; auto.
-    apply eps0_mult_spec.
-  Qed.
-
-  (** This one is stronger because it does not need any relation between e and f *)
-  Fact eps0_mult_right a e n f :
-      0₀ <ε₀ e
-    → a *₀ (ω^⟨e,n⟩ +₀ f)
-    = eps0_mpos (eps0_momega a e) n +₀ a *₀ f.
-  Proof.
-    intros He.
-    destruct f as [ | f i g H _ _ ] using eps0_head_rect.
-    + rewrite eps0_mult_head_right; auto.
-    + destruct (eps0_lt_sdec e f).
-      * rewrite eps0_add_head_lt', eps0_mult_head_right,
-             <- eps0_add_assoc, eps0_mpos_add_momega; auto.
-        eapply eps0_lt_trans; eassumption.
-      * rewrite eps0_add_head_eq', 
-               !eps0_mult_head_right,
-             <- eps0_add_assoc,
-                eps0_mpos_plus; auto.
-      * rewrite eps0_mult_head_right; auto.
-        apply eps0_add_below_omega.
-        - now apply eps0_exp_S_mono_left.
-        - apply eps0_lt_trans with (1 := H),
-                eps0_omega_mono_lt; auto.
-  Qed.
-
-  Fact eps0_mpos_momega_eq a n e :
-      0₀ <ε₀ e
-    → eps0_mpos (eps0_momega a e) n = a *₀ ω^⟨e,n⟩.
-  Proof.
-    intro.
-    rewrite <- (eps0_add_zero_right ω^⟨_,_⟩),
-                eps0_mult_right,
-                eps0_mult_zero_right,
-                eps0_add_zero_right; auto.
-  Qed.
-
-  Fact eps0_momega_eq a e :
-      0₀ <ε₀ e
-    → eps0_momega a e = a *₀ ω^e.
-  Proof.
-    intro; unfold eps0_omega.
-    rewrite <- eps0_mpos_momega_eq, eps0_mpos_O; auto.
-  Qed.
-
-  Fact eps0_mult_zero_left e : 0₀ *₀ e = 0₀.
-  Proof.
-    induction e as [ | n | e n f He Hf _ IHf ] using eps0_head_pos_rect.
-    + now rewrite eps0_mult_zero_right.
-    + now rewrite eps0_mult_pos_right, eps0_mpos_fix_0.
-    + rewrite eps0_mult_head_right, IHf; auto.
-      now rewrite eps0_momega_fix_0, eps0_mpos_fix_0, eps0_add_zero_left.
-  Qed.
-
-  Fact eps0_mult_distr a b c : a *₀ (b +₀ c) = a *₀ b +₀ a *₀ c.
-  Proof.
-    induction b as [ | n | e n f He Hf IHe IHf ] in a, c |- *
-      using eps0_head_pos_rect.
-    + now rewrite  eps0_mult_zero_right, !eps0_add_zero_left.
-    + destruct c as [ | k | c k g ? ? _ _ ] using eps0_head_pos_rect.
-      * now rewrite eps0_mult_zero_right, !eps0_add_zero_right.
-      * now rewrite eps0_add_exp_S, !eps0_mult_pos_right, eps0_mpos_plus.
-      * rewrite eps0_add_head_lt',
-                eps0_mult_head_right,
-                eps0_mult_pos_right,
-             <- eps0_add_assoc,
-                eps0_add_mpos_momega; auto.
-    + rewrite eps0_mult_right,
-             !eps0_add_assoc,
-           <- IHf, eps0_mult_right; auto.
-  Qed.
-
-  Fact eps0_mult_gt_zero a e :
-      0₀ <ε₀ a → 0₀ <ε₀ e → 0₀ <ε₀ a *₀ e.
-  Proof.
-    intros Ha He.
-    induction e as [ | n | e n f H1 H2 IH1 IH2 ] using eps0_head_pos_rect.
-    + now apply eps0_lt_irrefl in He.
-    + rewrite eps0_mult_pos_right; now apply eps0_mpos_gt_zero.
-    + rewrite eps0_mult_right; auto.
-      destruct (eps0_zero_or_pos f) as [ -> | Hf ].
-      * rewrite eps0_mult_zero_right, eps0_add_zero_right.
-        apply eps0_mpos_gt_zero.
-        apply eps0_lt_le_trans with (2 := eps0_momega_lt_pos Ha H1); auto.
-      * apply eps0_lt_le_trans with (1 := IH2 Hf); auto.
-  Qed.
-
-  (* Easy using substraction *)
-  Fact eps0_mult_mono_right a e f :
-      0₀ <ε₀ a → e <ε₀ f → a *₀ e <ε₀ a *₀ f.
-  Proof.
-    intros ? (? & -> & ?)%eps0_lt_inv_add.
-    rewrite eps0_mult_distr.
-    now apply eps0_add_incr, eps0_mult_gt_zero.
-  Qed.
-
-  Fact eps0_mult_mono_left a b e :
-      a <ε₀ b → a *₀ e ≤ε₀ b *₀ e.
-  Proof.
-    intros Hab.
-    induction e as [ | n | e n g H1 IH1 IH2 ] using eps0_head_pos_rect.
-    + rewrite !eps0_mult_zero_right; auto.
-    + rewrite !eps0_mult_pos_right.
-      left; apply eps0_mpos_mono_left; auto.
-    + rewrite !eps0_mult_right; auto.
-      apply eps0_add_mono; auto.
-      apply eps0_mpos_mono; auto.
-      apply eps0_momega_mono_left; auto.
-  Qed.
-
-  Fact eps0_mult_mono a b e f :
-      a ≤ε₀ b → e ≤ε₀ f → a *₀ e ≤ε₀ b *₀ f.
-  Proof.
-    destruct (eps0_zero_or_pos a) as [ -> | Ha ].
-    1: rewrite eps0_mult_zero_left; auto.
-    intros [ H1 | <- ] [ H2 | <- ].
-    + apply eps0_le_trans with (a *₀ f).
-      * left; apply eps0_mult_mono_right; auto.
-      * now apply eps0_mult_mono_left.
-    + now apply eps0_mult_mono_left.
-    + left; now apply eps0_mult_mono_right.
-    + now right.
-  Qed.
-
-  Fact eps0_mult_head a i b e j f :
-      0₀ <ε₀ e
-    → b <ε₀ ω^a
-    → f <ε₀ ω^e
-    → (ω^⟨a,i⟩ +₀ b) *₀ (ω^⟨e,j⟩ +₀ f)
-     = ω^⟨a+₀e,j⟩ +₀ (ω^⟨a,i⟩ +₀ b) *₀ f.
-  Proof.
-    intros; rewrite eps0_mult_right, eps0_momega_fix_1, eps0_mpos_omega; auto.
-  Qed.
-
-  Fact eps0_mult_head_exp_S a i b e j :
-      0₀ <ε₀ e → b <ε₀ ω^a → (ω^⟨a,i⟩ +₀ b) *₀ ω^⟨e,j⟩ = ω^⟨a+₀e,j⟩.
-  Proof.
-    intros H1 H2.
-    rewrite <- (eps0_add_zero_right ω^⟨_,j⟩), eps0_mult_head; auto.
-    now rewrite eps0_mult_zero_right, eps0_add_zero_right.
-  Qed.
-
-  Fact eps0_mult_exp_S_head a i e j f : 
-      0₀ <ε₀ e
-    → f <ε₀ ω^e
-    → ω^⟨a,i⟩ *₀ (ω^⟨e,j⟩ +₀ f)
-    = ω^⟨a+₀e,j⟩ +₀ ω^⟨a,i⟩ *₀ f.
-  Proof. intros; rewrite <- (eps0_add_zero_right ω^⟨_,i⟩), eps0_mult_head; auto. Qed.
-
-  Fact eps0_mult_omega_head a e j f : 
-      0₀ <ε₀ e
-    → f <ε₀ ω^e
-    → ω^a *₀ (ω^⟨e,j⟩ +₀ f)
-    = ω^⟨a+₀e,j⟩ +₀ ω^a *₀ f.
-  Proof. apply eps0_mult_exp_S_head. Qed.
-
-  Fact eps0_mult_exp_S_pos e i j : ω^⟨e,i⟩ *₀ ω^⟨0₀,j⟩ = ω^⟨e,i*j+i+j⟩.
-  Proof. now rewrite eps0_mult_pos_right, eps0_mpos_exp_S. Qed.
-
-  Fact eps0_mult_exp_S e i f j : 0₀ <ε₀ f → ω^⟨e,i⟩ *₀ ω^⟨f,j⟩ = ω^⟨e+₀f,j⟩.
-  Proof. intro; rewrite <- (eps0_add_zero_right ω^⟨e,i⟩), eps0_mult_head_exp_S; auto. Qed.
-
-  Fact eps0_mult_exp_S_omega e i f : 0₀ <ε₀ f → ω^⟨e,i⟩ *₀ ω^f = ω^(e+₀f).
-  Proof. intro; apply eps0_mult_exp_S; auto. Qed.
-
-  Fact eps0_mult_omega_exp_S e f n: ω^e *₀ ω^⟨f,n⟩ = ω^⟨e+₀f,n⟩.
-  Proof.
-    unfold eps0_omega.
-    destruct (eps0_zero_or_pos f) as [ -> | ].
-    + now rewrite eps0_mult_exp_S_pos, eps0_add_zero_right.
-    + rewrite eps0_mult_exp_S; auto.
-  Qed.
-
-  Fact eps0_mult_omega e f : ω^e *₀ ω^f = ω^(e+₀f).
-  Proof. apply eps0_mult_omega_exp_S. Qed.
-
-  (** From ω^e.n.ω^f = ω^(e+f) *)
-  Fact eps0_mult_below_omega a b e n f : 
-      a <ε₀ ω^⟨e,n⟩
-    → b <ε₀ ω^f
-    → a *₀ b <ε₀ ω^(e+₀f).
-  Proof.
-    intros H1 H2.
-    apply eps0_le_lt_trans with (ω^⟨e,n⟩ *₀ b).
-    + apply eps0_mult_mono; auto.
-    + destruct (eps0_zero_or_pos f) as [ -> | ].
-      * apply eps0_lt_one in H2 as ->.
-        rewrite eps0_mult_zero_right; auto.
-      * rewrite <- eps0_mult_exp_S_omega with (i := n); auto.
-        apply eps0_mult_mono_right; auto.
-  Qed.
-
-  Remark eps0_mult_below_omega_1 a b e f : 
-      a <ε₀ ω^e → b <ε₀ ω^f → a *₀ b <ε₀ ω^(e+₀f).
-  Proof. apply eps0_mult_below_omega. Qed.
-
-  Fact eps0_mult_mpos a b n : eps0_mpos (a *₀ b) n = a *₀ eps0_mpos b n. 
-  Proof.
-    induction b using eps0_head_pos_rect in a, n |- *.
-    + now rewrite eps0_mult_zero_right, eps0_mpos_fix_0, eps0_mult_zero_right.
-    + now rewrite eps0_mpos_exp_S, !eps0_mult_pos_right, eps0_mpos_mult.
-    + rewrite eps0_mult_distr.
-      destruct a as [ | ] using eps0_head_rect.
-      * now rewrite !eps0_mult_zero_left, eps0_add_zero_left, eps0_mpos_fix_0.
-      * rewrite eps0_mult_head_exp_S, !eps0_mpos_fix_1; auto.
-        - rewrite eps0_mult_distr, eps0_mult_head_exp_S; auto.
-        - apply eps0_mult_below_omega with (n := i0 +ₚ 1ₚ); auto.
-          rewrite <- eps0_add_exp_S; auto.
-  Qed.
-
-  (** This one was a long shot !! 
-      induction on c and case analysis on b and a *)
-  Theorem eps0_mult_assoc a b c : a *₀ (b *₀ c) = (a *₀ b) *₀ c.
-  Proof.
-    induction c as [ | n | e n f He Hf IHe IHf ]
-      in a, b |- * using eps0_head_pos_rect.
-    + now rewrite !eps0_mult_zero_right.
-    + now rewrite !eps0_mult_pos_right, eps0_mult_mpos.
-    + destruct b as [ | i | g i h Hg Hh _ ] using eps0_head_pos_rect.
-      * rewrite eps0_mult_zero_left,
-               !eps0_mult_zero_right,
-                eps0_mult_zero_left; auto.
-      * rewrite eps0_mult_exp_S_head,
-                eps0_add_zero_left, 
-               !eps0_mult_distr,
-                IHf,
-                eps0_mult_pos_right,
-            <- !eps0_mpos_momega_eq,
-                eps0_momega_mpos; auto.
-      * rewrite eps0_mult_head, eps0_mult_distr, IHf; auto.
-        destruct a as [ | u j v Hu _ _ ] using eps0_head_rect.
-        - now rewrite !eps0_mult_zero_left, eps0_add_zero_left.
-        - rewrite eps0_mult_head_exp_S; auto.
-          2: apply eps0_lt_le_trans with (1 := He); auto.
-          rewrite !eps0_mult_head, eps0_add_assoc; auto.
-          apply eps0_mult_below_omega with (n := j +ₚ 1ₚ); auto.
-          apply eps0_lt_le_trans with (ω^⟨u,j⟩ +₀ ω^u); auto.
-          unfold eps0_omega; rewrite eps0_add_exp_S; auto.
-  Qed.
-
-  Fact eps0_mult_one_left e : 1₀ *₀ e = e.
-  Proof.
-    rewrite <- eps0_omega_zero.
-    induction e using eps0_head_pos_rect.
-    + now rewrite eps0_mult_zero_right.
-    + now rewrite eps0_mult_pos_right, eps0_mpos_omega.
-    + unfold eps0_omega.
-      rewrite eps0_mult_exp_S_head, eps0_add_zero_left; auto.
-      f_equal; auto.
-  Qed.
-
-  Fact eps0_mult_one_right e : e *₀ 1₀ = e.
-  Proof.
-    rewrite <- eps0_omega_zero; unfold eps0_omega.
-    now rewrite eps0_mult_pos_right, eps0_mpos_O.
-  Qed.
-
-  Fact eps0_mult_zero_inv a e : a *₀ e = 0₀ → a = 0₀ ∨ e = 0₀.
-  Proof.
-    intros E.
-    destruct (eps0_zero_or_pos a) as [ | Ha ]; auto.
-    destruct (eps0_zero_or_pos e) as [ | He ]; auto.
-    destruct (@eps0_lt_irrefl 0₀).
-    rewrite <- E at 2.
-    now apply eps0_mult_gt_zero.
-  Qed.
-
-  Fact eps0_mult_cancel a e f : 0₀ <ε₀ a → a *₀ e = a *₀ f → e = f.
-  Proof.
-    intros Ha H.
-    destruct (eps0_lt_sdec e f) as [ e f C | | e f C ]; auto; exfalso;
-      apply (@eps0_lt_irrefl (a *₀ e)).
-    + rewrite H at 2; now apply eps0_mult_mono_right.
-    + rewrite H at 1; now apply eps0_mult_mono_right.
-  Qed.
-
-  Fact eps0_mult_succ_right a e : a *₀ (S₀ e) = a *₀ e +₀ a.
-  Proof. now rewrite <- eps0_add_one_right, eps0_mult_distr, eps0_mult_one_right. Qed.
-
-End eps0_mult.
-
-Infix "*₀" := eps0_mult.
-
-(* 0.a = a.0 = 0 *)
-Check eps0_mult_zero_left.
-Check eps0_mult_zero_right.
-(* 1.a = a.1 = 0 *)
-Check eps0_mult_one_left.
-Check eps0_mult_one_right.
-(* a.b = 0 → a = 0 ∨ b = 0 *)
-Check eps0_mult_zero_inv.
-(* a.(b.c) = (a.b).c *)
-Check eps0_mult_assoc.
-(* 0 < e -> a < b -> e.a < e.b *)
-Check eps0_mult_mono_right.
-(* Continuity is missing e.(lub P) = lub e.P *)
-Check eps0_mult_mono.
-Check eps0_mult_distr.
-Check eps0_mult_cancel.
-
-(** Section expo *)
-
-Fact eps0_omega_succ e : ω^(S₀ e) = ω^e *₀ ω^1₀.
-Proof.
-  now rewrite <- eps0_succ_zero_is_one,
-                 eps0_mult_omega,
-                 eps0_succ_zero_is_one,
-                 eps0_add_one_right.
-Qed.
-
-Check eps0_omega_zero.
-Check eps0_omega_succ.
-
-Section eps0_exponentiation.
-
-  (** Define exponentiation in CNF 
-   
-      The formula here: 
-
-         https://proofwiki.org/wiki/Ordinal_Exponentiation_via_Cantor_Normal_Form/Limit_Exponents
-
-      (w^a₁.n₁+...+w^aₚ.nₚ)^e = w^(a₁.e) when a₁ > ... > aₚ 
-  *)
-
-  Inductive eps0_expo_gr α : ε₀ → ε₀ → Prop :=
-    | eps0_expr_gr_0 : eps0_expo_gr α 0₀ 0₀
-    | eps0_expr_gr_1 γ n β : β <ε₀ ω^γ → eps0_expo_gr α (ω^⟨γ,n⟩ +₀ β) ω^(γ*₀α).
-
-  Fact eps0_expo_fun α e1 f1 e2 f2 :
-    eps0_expo_gr α e1 f1 → eps0_expo_gr α e2 f2 → e1 = e2 → f1 = f2.
-  Proof.
-    intros [] []; auto.
-    + now intros ?%eps0_zero_neq_head.
-    + symm; now intros ?%eps0_zero_neq_head.
-    + intros (<- & <- & <-)%eps0_head_split_uniq; auto.
-  Qed. 
-
-  Definition eps0_expo_pwc e α : sig (eps0_expo_gr α e).
-  Proof.
-    destruct e as [ | e ] using eps0_head_rect.
-    + exists 0₀; constructor.
-    + exists ω^(e*₀α); constructor; auto.
-  Qed.
-
-  Definition eps0_expo e α := proj1_sig (eps0_expo_pwc e α).
-
-  Fact eps0_expo_spec e α : eps0_expo_gr α e (eps0_expo e α).
-  Proof. apply (proj2_sig _). Qed.
-
-  Hint Constructors eps0_expo_gr : core.
-  Hint Resolve eps0_expo_spec : core.
-
-  Tactic Notation "functionality" :=
-    apply eps0_expo_fun with (1 := eps0_expo_spec _ _) (3 := eq_refl); auto.
-
-  Fact eps0_expo_zero e : eps0_expo 0₀ e = 0₀.
-  Proof. functionality; constructor. Qed.
-
-  Fact eps0_expo_head a n b e : b <ε₀ ω^a → eps0_expo (ω^⟨a,n⟩ +₀ b) e = ω^(a*₀e).
-  Proof. intros; functionality; constructor; auto. Qed.
-
-  Fact eps0_expo_exp_S a n e : eps0_expo ω^⟨a,n⟩ e = ω^(a*₀e).
-  Proof. rewrite <- (eps0_add_zero_right ω^⟨_,n⟩), eps0_expo_head; auto. Qed.
-
-  Fact eps0_expo_omega_pos n e : eps0_expo ω^⟨1₀,n⟩ e = ω^e.
-  Proof. now rewrite eps0_expo_exp_S, eps0_mult_one_left. Qed.
-
-  Fact eps0_expo_omega a e : eps0_expo ω^a e = ω^(a*₀e).
-  Proof. apply eps0_expo_exp_S. Qed.
-
-  (** Need to check more equations *)
-
-End eps0_exponentiation.
 
 (* Hence a successor is not a limit ordinal 
 
@@ -1637,7 +885,7 @@ Definition eps0_is_succ e := ∃f, e = S₀ f.
 Fact eps0_is_succ_S e : eps0_is_succ (S₀ e).
 Proof. now exists e. Qed.
 
-Hint Resolve eps0_is_succ_S : core.
+#[local] Hint Resolve eps0_is_succ_S : core.
 
 Fact eps0_is_succ_iff e : eps0_is_succ e ↔ E0_is_succ (π₁ e).
 Proof.
@@ -1647,16 +895,14 @@ Proof.
     apply eps0_eq_iff; now rewrite H1.
 Qed.
 
-Fact eps0_is_succ_exp_S n : eps0_is_succ ω^⟨0₀,n⟩.
+Fact eps0_is_succ_exp_zero n : eps0_is_succ ω^⟨0₀,n⟩.
 Proof.
   destruct (pos_one_or_succ n) as [ -> | (m & ->) ].
-  + exists 0₀.
-    rewrite eps0_succ_zero_is_one; apply eps0_omega_zero.
-  + exists ω^⟨0₀,m⟩. 
-    now rewrite eps0_succ_exp_S.
+  + exists 0₀; rewrite eps0_succ_zero_is_one; apply eps0_omega_zero.
+  + exists ω^⟨0₀,m⟩; now rewrite eps0_succ_exp.
 Qed.
 
-Hint Resolve eps0_is_succ_exp_S : core.
+#[local] Hint Resolve eps0_is_succ_exp_zero : core.
 
 Definition eps0_is_limit e := e ≠ 0₀ ∧ ¬ eps0_is_succ e.
 
@@ -1682,7 +928,7 @@ Proof.
   now intros [ [] _ ].
 Qed.
 
-Hint Resolve eps0_is_limit_pos : core.
+#[local] Hint Resolve eps0_is_limit_pos : core.
 
 Fact eps0_add_is_limit_inv a e :
     eps0_is_limit (a +₀ e)
@@ -1716,7 +962,7 @@ Proof.
   now intros ?%eps0_lt_irrefl.
 Qed.
 
-Fact eps0_is_limit_exp_S e n : e ≠ 0₀ → eps0_is_limit ω^⟨e,n⟩.
+Fact eps0_is_limit_exp e n : e ≠ 0₀ → eps0_is_limit ω^⟨e,n⟩.
 Proof.
   intros H.
   apply eps0_is_limit_iff.
@@ -1725,47 +971,38 @@ Proof.
   contradict H; now apply eps0_eq_iff.
 Qed.
 
-Fact eps0_is_limit_exp_S_iff e n : eps0_is_limit ω^⟨e,n⟩ ↔ e ≠ 0₀.
+Fact eps0_is_limit_exp_iff e n : eps0_is_limit ω^⟨e,n⟩ ↔ e ≠ 0₀.
 Proof.
   split.
   + intros [ _ H1 ] ->; apply H1; auto.
-  + apply eps0_is_limit_exp_S.
+  + apply eps0_is_limit_exp.
 Qed.
 
 Fact eps0_is_limit_omega e : e ≠ 0₀ → eps0_is_limit ω^e.
-Proof. apply eps0_is_limit_exp_S. Qed.
+Proof. apply eps0_is_limit_exp. Qed.
 
-Fact eps0_is_limit_add_omega a e : e ≠ 0₀ → eps0_is_limit (a +₀ ω^e).
+Fact eps0_is_limit_tf a e : e ≠ 0₀ → eps0_is_limit (a +₀ ω^e).
 Proof. intro; apply eps0_add_is_limit, eps0_is_limit_omega; auto. Qed.
 
-Fact eps0_add_omega_not_zero a e : 0₀ ≠ a +₀ ω^e.
+Fact eps0_tf_not_zero a e : 0₀ ≠ a +₀ ω^e.
 Proof.
   intros H.
   apply (@eps0_lt_irrefl (a+₀ω^e)).
   rewrite <- H at 1.
-  apply eps0_lt_le_trans with (1 := eps0_zero_lt_omega e).
-  rewrite <- (eps0_add_zero_left ω^e) at 1.
-  apply eps0_add_mono_left, eps0_zero_least.
+  apply eps0_lt_le_trans with (1 := eps0_zero_lt_omega e); auto.
+Qed.
+
+Fact eps0_succ_eq_tf a b e : S₀ a = b +₀ ω^e → e = 0₀ ∧ a = b.
+Proof.
+  rewrite <- eps0_add_one_right, <- eps0_omega_zero; intros H.
+  destruct eps0_tf_fun_right with (1 := H); split; auto.
+  rewrite eps0_omega_zero, !eps0_add_one_right in H.
+  now apply eps0_succ_inj.
 Qed.
 
 Fact eps0_add_omega_not_succ a b e : e ≠ 0₀ → S₀ a ≠ b +₀ ω^e.
-Proof.
-  intros E H.
-  assert (eps0_is_limit (S₀ a)) as [ _ [] ]; eauto.
-  rewrite H.
-  now apply eps0_is_limit_add_omega.
-Qed.
+Proof. intros H; contradict H; now apply eps0_succ_eq_tf in H. Qed.
 
-Fact eps0_succ_eq_add_omega a b e : S₀ a = b +₀ ω^e → e = 0₀.
-Proof.
-  intros H.
-  destruct (eps0_eq_dec e 0₀); auto.
-  now apply eps0_add_omega_not_succ in H.
-Qed.
-
-Fact eps0_succ_eq_omega a e : S₀ a = ω^e → e = 0₀.
-Proof.
-  rewrite <- (eps0_add_zero_left ω^e).
-  apply eps0_succ_eq_add_omega.
-Qed.
+Fact eps0_succ_eq_omega a e : S₀ a = ω^e → e = 0₀ ∧ a = 0₀.
+Proof. rewrite <- (eps0_add_zero_left ω^e); apply eps0_succ_eq_tf. Qed.
 
