theories/eps0_fseq.v
@@ -8,14 +8,14 @@
 (**************************************************************)
 
 From Coq Require Import List Relations Arith Lia Wellfounded Utf8.
-From Hydra Require Import utils pos eps0 eps0_least_split.
+From Hydra Require Import utils pos eps0 eps0_ltf eps0_mult.
 
 Set Implicit Arguments.
 
 #[local] Notation π₁ := proj1_sig.
 #[local] Notation π₂ := proj2_sig.
 
-Section eps0_tail_rect.
+Section eps0_ltf_pos_rect.
 
   (** Induction principle corresponding to the following building rules 
       for ordinals below ε₀:
@@ -28,22 +28,24 @@ Section eps0_tail_rect.
   Variables (P : ε₀ → Type)
             (HP0 : P 0₀)
             (HP1 : ∀ e, P e → P (S₀ e))
-            (HP2 : ∀ g e, e ≠ 0₀ → eps0_least_split g e → P g → P e → P (g +₀ ω^e)).
+            (HP2 : ∀ g e, e ≠ 0₀ → eps0_ltf g e → P g → P e → P (g +₀ ω^e)).
 
-  Theorem eps0_tail_rect e : P e.
+  Theorem eps0_ltf_pos_rect e : P e.
   Proof.
-    induction e as [ | e f H IH ] using eps0_least_split_rect; auto.
+    induction e as [ | e f H IH ] using eps0_ltf_rect; auto.
     destruct (eps0_zero_or_pos f) as [ -> | Hf ].
     + rewrite eps0_omega_zero, eps0_add_one_right; auto.
     + apply HP2; auto.
       intros ->; now apply eps0_lt_irrefl in Hf.
   Qed.
 
-End eps0_tail_rect.
+End eps0_ltf_pos_rect.
 
-Corollary eps0_least_split_find e : eps0_is_limit e → { a : _ & { g | e = a+₀ω^g ∧ g ≠ 0₀ ∧ eps0_least_split a g } }.
+#[local] Hint Resolve eps0_is_succ_S : core.
+
+Corollary eps0_ltf_find e : eps0_is_limit e → { a : _ & { g | e = a+₀ω^g ∧ g ≠ 0₀ ∧ eps0_ltf a g } }.
 Proof.
-  destruct e as [ | | a g ] using eps0_tail_rect.
+  destruct e as [ | | a g ] using eps0_ltf_pos_rect.
   + now intros [ [] _ ].
   + intros [ _ [] ]; auto.
   + exists a, g; auto.
@@ -56,212 +58,122 @@ Section eps0_discriminate.
             (HP1 : ∀ e, P (S₀ e))
             (HP2 : ∀ e, eps0_is_limit e → P e).
 
-  Hint Resolve eps0_is_limit_add_omega : core.
-            
+  Hint Resolve eps0_is_limit_tf : core.
+
   Theorem eps0_discriminate e : P e.
-  Proof. destruct e using eps0_tail_rect; auto. Qed.
+  Proof. destruct e using eps0_ltf_pos_rect; auto. Qed.
 
 End eps0_discriminate.
 
-(** Tailored induction principle for computing the fundemental sequence *)
+(** Tailored dependent induction principle for computing the fundemental sequence *)
 
-Section eps0_fseq_rect.
+Section eps0_fseq_dep_rect.
 
-  Variables (P : forall e, eps0_is_limit e → Type)
-            (HP0 : ∀ g e l, eps0_least_split g (S₀ e) → @P (g +₀ ω^(S₀ e)) l)
-            (HP1 : ∀ g e l l', eps0_least_split g e → @P e l → @P (g +₀ ω^e) l').
+  Variables (P : ∀e, eps0_is_limit e → Type)
+            (HP0 : ∀ g e l, eps0_ltf g (S₀ e) → @P (g +₀ ω^(S₀ e)) l)
+            (HP1 : ∀ g e l l', eps0_ltf g e → @P e l → @P (g +₀ ω^e) l').
 
-  Hint Resolve eps0_is_limit_add_omega : core.
+  Hint Resolve eps0_is_limit_tf : core.
 
-  Theorem eps0_fseq_rect e (l : eps0_is_limit e) : P l.
+  Theorem eps0_fseq_dep_rect e (l : eps0_is_limit e) : P l.
   Proof.
     revert l.
     destruct e as [ | e | g e H1 H2 _ _ ]
-      using eps0_tail_rect.
+      using eps0_ltf_pos_rect.
     + now intros [ [] _ ].
     + intros [ _ [] ]; eauto.
     + induction e as [ | e | h e H3 H4 _ IH ]
         in H1, g, H2 |- *
-        using eps0_tail_rect; intros l.
+        using eps0_ltf_pos_rect; intros l.
       * now destruct H1.
       * now apply HP0.
       * assert (eps0_is_limit (h+₀ ω^(e))) as l' by auto.
         apply HP1 with l'; auto.
   Qed.
 
-End eps0_fseq_rect.
+End eps0_fseq_dep_rect.
 
 (** We build the fundemental sequence *)
 
-Inductive eps0_fseq_gr : ε₀ → (nat → ε₀) → Prop :=
-  | eps0_fseq_gr_0 g b   : eps0_least_split g (S₀ b)
-                         → eps0_fseq_gr (g +₀ ω^(S₀ b)) (λ n, g +₀ ω^⟨b,n⟩)
-  | eps0_fseq_gr_1 g b r : eps0_is_limit b
-                         → eps0_least_split g b
-                         → eps0_fseq_gr b r
-                         → eps0_fseq_gr (g +₀ ω^b) (λ n, g +₀ ω^(r n)).
+Section eps0_fseq.
 
-Local Lemma eps0_fseq_gr_fun_rec e se f sf :
-  eps0_fseq_gr e se → eps0_fseq_gr f sf → e = f → ∀n, se n = sf n.
-Proof.
-  intros H; revert H f sf.
-  induction 1 as [ g b Hs | g b r H0 Hs H1 IH1 ].
-  + induction 1 as [ g' b' Hs' | g' b' r' H0' Hs' H2 IH2 ].
-    * intros (<- & <-%eps0_succ_inj)%eps0_split_least_uniq; auto.
-    * intros <-%eps0_add_omega_fun_right; eauto.
-      destruct H0' as (_ & []); eauto.
-  + induction 1 as [ g' b' Hs' | g' b' r' H0' Hs' H2 IH2 ].
-    * intros ->%eps0_add_omega_fun_right; eauto.
-      destruct H0 as (_ & []); eauto.
-    * intros (<- & <-)%eps0_split_least_uniq; auto.
-      intro; now rewrite IH1 with (1 := H2).
-Qed.
+  Inductive eps0_fseq_gr : ε₀ → (nat → ε₀) → Prop :=
+    | eps0_fseq_gr_0 g b   : eps0_ltf g (S₀ b)
+                           → eps0_fseq_gr (g +₀ ω^(S₀ b)) (λ n, g +₀ ω^⟨b,n⟩)
+    | eps0_fseq_gr_1 g b r : eps0_is_limit b
+                           → eps0_ltf g b
+                           → eps0_fseq_gr b r
+                           → eps0_fseq_gr (g +₀ ω^b) (λ n, g +₀ ω^(r n)).
 
-Lemma eps0_fseq_gr_fun e r r' : eps0_fseq_gr e r → eps0_fseq_gr e r' → ∀n, r n = r' n.
-Proof. intros H1 H2; now apply (eps0_fseq_gr_fun_rec H1 H2). Qed.
+  Hint Constructors eps0_fseq_gr : core.
 
-(** By WF induction, we build the fundemental sequence of a limit
-    ordinal, packed with conformity (pwc) as spec'd with eps0_fseq_gr *)
-Theorem eps0_fseq_pwc e : eps0_is_limit e → sig (eps0_fseq_gr e).
-Proof.
-  induction 1 as [ g e l H | g e l l' H (lam & Hlam) ] using eps0_fseq_rect.
-  + exists (λ n, g +₀ ω^⟨e,n⟩); now constructor.
-  + exists (λ n, g +₀ ω^(lam n)); constructor; auto.
-Qed.
+  Local Lemma eps0_fseq_gr_fun_rec e se f sf :
+    eps0_fseq_gr e se → eps0_fseq_gr f sf → e = f → ∀n, se n = sf n.
+  Proof.
+    intros H; revert H f sf.
+    induction 1 as [ g b Hs | g b r H0 Hs H1 IH1 ].
+    + induction 1 as [ g' b' Hs' | g' b' r' H0' Hs' H2 IH2 ].
+      * intros (<- & <-%eps0_succ_inj)%eps0_eq_ltf_inv; auto.
+      * intros <-%eps0_tf_fun_right; eauto.
+        destruct H0' as (_ & []); eauto.
+    + induction 1 as [ g' b' Hs' | g' b' r' H0' Hs' H2 IH2 ].
+      * intros ->%eps0_tf_fun_right; eauto.
+        destruct H0 as (_ & []); eauto.
+      * intros (<- & <-)%eps0_eq_ltf_inv; auto.
+        intro; now rewrite IH1 with (1 := H2).
+  Qed.
 
-Definition eps0_fseq {e} (l : eps0_is_limit e) := π₁ (@eps0_fseq_pwc e l).
+  Lemma eps0_fseq_gr_fun e r r' : eps0_fseq_gr e r → eps0_fseq_gr e r' → ∀n, r n = r' n.
+  Proof. intros H1 H2; now apply (eps0_fseq_gr_fun_rec H1 H2). Qed.
 
-Fact eps0_fseq_spec e l : eps0_fseq_gr e (@eps0_fseq e l).
-Proof. apply (proj2_sig _). Qed.
+  (** We build the fundemental sequence of a limit ordinal, packed 
+      with conformity (pwc) as spec'd with eps0_fseq_gr *)
+  Definition eps0_fseq_pwc e : eps0_is_limit e → sig (eps0_fseq_gr e).
+  Proof.
+    induction 1 as [ g e l | g e l l' ? (lam & ?) ] using eps0_fseq_dep_rect.
+    + exists (λ n, g +₀ ω^⟨e,n⟩); now constructor.
+    + exists (λ n, g +₀ ω^(lam n)); constructor; auto.
+  Qed.
 
-Fact eps0_fseq_pirr e (l l' : eps0_is_limit e) n :
-    eps0_fseq l n = eps0_fseq l' n.
-Proof. revert n; apply eps0_fseq_gr_fun with e; apply eps0_fseq_spec. Qed.
+  Definition eps0_fseq {e} (l : eps0_is_limit e) := π₁ (@eps0_fseq_pwc e l).
 
-Fact eps0_fseq_fix_0 g e (l : eps0_is_limit (g +₀ ω^(S₀ e))) n :
-    eps0_least_split g (S₀ e)
-  → eps0_fseq l n = g +₀ ω^⟨e,n⟩.
-Proof.
-  intro.
-  revert n; apply eps0_fseq_gr_fun with (1 := eps0_fseq_spec _).
-  constructor; auto.
-Qed.
+  Fact eps0_fseq_spec e l : eps0_fseq_gr e (@eps0_fseq e l).
+  Proof. apply (proj2_sig _). Qed.
 
-Fact eps0_fseq_fix_1 g e (l : eps0_is_limit (g +₀ ω^e))
-                         (l' : eps0_is_limit e) n :
-    eps0_least_split g e
-  → eps0_fseq l n = g +₀ ω^(eps0_fseq l' n).
-Proof.
-  intros H.
-  revert n; apply eps0_fseq_gr_fun with (1 := eps0_fseq_spec _).
-  constructor; auto.
-  apply eps0_fseq_spec.
-Qed.
+  Fact eps0_fseq_pirr e (l l' : eps0_is_limit e) n : eps0_fseq l n = eps0_fseq l' n.
+  Proof. revert n; apply eps0_fseq_gr_fun with e; apply eps0_fseq_spec. Qed.
 
-#[local] Hint Resolve
-     eps0_least_split_zero 
-     eps0_least_split_exp_S
-     eps0_least_split_add_exp_S : core.
+  Fact eps0_fseq_fix_0 g e (l : eps0_is_limit (g +₀ ω^(S₀ e))) n :
+    eps0_ltf g (S₀ e) → eps0_fseq l n = g +₀ ω^⟨e,n⟩.
+  Proof.
+    intro.
+    revert n; apply eps0_fseq_gr_fun with (1 := eps0_fseq_spec _).
+    constructor; auto.
+  Qed.
 
-Fact eps0_fseq_omega_succ e (l : eps0_is_limit ω^(S₀ e)) n :
-    eps0_fseq l n = ω^⟨e,n⟩.
-Proof.
-  revert l; rewrite <- (eps0_add_zero_left ω^_); intros l.
-  rewrite eps0_fseq_fix_0; auto.
-  now rewrite eps0_add_zero_left.
-Qed.
+  Fact eps0_fseq_fix_1 g e (l : eps0_is_limit (g +₀ ω^e))
+                           (l' : eps0_is_limit e) n :
+    eps0_ltf g e → eps0_fseq l n = g +₀ ω^(eps0_fseq l' n).
+  Proof.
+    intros H.
+    revert n; apply eps0_fseq_gr_fun with (1 := eps0_fseq_spec _).
+    constructor; auto.
+    apply eps0_fseq_spec.
+  Qed.
 
-Fact eps0_fseq_omega_is_limit e (l : eps0_is_limit ω^e) (l' : eps0_is_limit e) n :
-    eps0_fseq l n = ω^(eps0_fseq l' n).
-Proof.
-  revert l; rewrite <- (eps0_add_zero_left ω^_); intros l.
-  rewrite eps0_fseq_fix_1 with (l' := l'); auto.
-  now rewrite eps0_add_zero_left.
-Qed.
+  Hint Resolve eps0_ltf_zero eps0_ltf_exp eps0_ltf_hnf : core.
 
-Fact eps0_head_least_split e g i f :
-    g <ε₀ ω^e
-  → ω^f <ε₀ ω^e
-  → eps0_least_split g f
-  → eps0_least_split (ω^⟨e,i⟩ +₀ g) f.
-Proof.
-  intros H1 H2 H3 b Hb.
-  destruct (eps0_le_lt_dec (ω^⟨e,i⟩ +₀ g) b) as [ | C ]; auto.
-  apply eps0_lt_add_inv_add in C as [ C | (k & -> & C) ].
-  - assert (b +₀ eps0_omega f <ε₀ ω^⟨e,i⟩) as D.
-    1:{ apply eps0_add_below_exp_S; auto. }
-    rewrite <- Hb, eps0_add_assoc in D.
-    now apply eps0_incr_not_lt in D.
-  - rewrite !eps0_add_assoc in Hb.
-    apply eps0_add_cancel, H3 in Hb.
-    destruct (@eps0_lt_irrefl k).
-    now apply eps0_lt_le_trans with (1 := C). 
-Qed.
+  (** The fundemental sequence is monotonic *)
+  Fact eps0_fseq_mono e (l : eps0_is_limit e) : ∀ n m, n < m → eps0_fseq l n <ε₀ eps0_fseq l m.
+  Proof.
+    induction l using eps0_fseq_dep_rect; intros n m Hnm.
+    + rewrite !eps0_fseq_fix_0; auto.
+      apply eps0_add_mono_right, eps0_exp_mono_right; auto.
+    + rewrite !eps0_fseq_fix_1 with (l' := l1); auto.
+      apply eps0_add_mono_right, eps0_omega_mono_lt; auto.
+  Qed.
 
-Fact eps0_exp_S_least_split e n : eps0_least_split ω^⟨e,n⟩ e.
-Proof.
-  intros b; rewrite eps0_add_exp_S_omega; intros Hb.
-  destruct (eps0_le_lt_dec ω^⟨e,n⟩ b) as [ | C ]; auto.
-  apply eps0_lt_exp_S_inv in C
-    as [ [ -> | (i & c & -> & H1 & H2) ] | (f & i & H1 & H2) ].
-  + rewrite eps0_add_zero_left in Hb.
-    now apply eps0_exp_S_inj, proj2 in Hb.
-  + rewrite eps0_add_assoc, eps0_add_lt_omega, eps0_add_exp_S_omega in Hb; auto.
-    apply eps0_exp_S_inj, proj2, pos_succ_inj in Hb; lia.
-  + rewrite eps0_add_lt_omega in Hb; auto.
-    * now apply eps0_exp_S_inj, proj2 in Hb.
-    * now apply eps0_lt_trans with (1 := H1),
-                eps0_exp_S_mono_left.
-Qed.
-
-Fact eps0_fseq_exp_S_succ_one e (l : eps0_is_limit ω^⟨S₀ e,1ₚ⟩) n :
-    eps0_fseq l n = ω^⟨e,n⟩.
-Proof. apply eps0_fseq_omega_succ. Qed.
-
-Fact eps0_fseq_exp_S_succ_succ e k (l : eps0_is_limit ω^⟨S₀ e,k +ₚ 1ₚ⟩) n :
-    eps0_fseq l n = ω^⟨S₀ e,k⟩ +₀ ω^⟨e,n⟩.
-Proof.
-  revert l; rewrite <- eps0_add_exp_S_omega; intros l.
-  rewrite eps0_fseq_fix_0; auto.
-Qed.
-
-Fact eps0_fseq_exp_S_one_is_limit e (l : eps0_is_limit ω^⟨e,1ₚ⟩) (l' : eps0_is_limit e) n :
-    eps0_fseq l n = ω^(eps0_fseq l' n).
-Proof. apply eps0_fseq_omega_is_limit. Qed.
-
-Fact eps0_fseq_exp_S_succ_is_limit e i (l : eps0_is_limit ω^⟨e,i +ₚ 1ₚ⟩) (l' : eps0_is_limit e) n :
-    eps0_fseq l n = ω^⟨e,i⟩ +₀ ω^(eps0_fseq l' n).
-Proof.
-  revert l; rewrite <- eps0_add_exp_S_omega; intros l.
-  rewrite eps0_fseq_fix_1 with (l' := l'); auto.
-Qed.
-
-(* Another computation for fseq :
-     fseq (ω^e.i +₀ f) n = ω^e.i + fseq f n
-   when f < ω^e *)
-Lemma eps0_fseq_head e i f (l : eps0_is_limit (ω^⟨e,i⟩ +₀ f)) (l' : eps0_is_limit f) n :
-    f <ε₀ ω^e → eps0_fseq l n = ω^⟨e,i⟩ +₀ eps0_fseq l' n.
-Proof.
-  intros Hf; revert l.
-  induction l' as [ g j h | ] using eps0_fseq_rect; rewrite <- eps0_add_assoc; intros l.
-  + rewrite !eps0_fseq_fix_0, eps0_add_assoc; auto.
-  + rewrite !eps0_fseq_fix_1 with (l' := l'1), eps0_add_assoc; auto.
-Qed.
-
-(** The fundemental sequence is monotonic *)
-Fact eps0_fseq_mono e (l : eps0_is_limit e) : ∀ n m, n < m → eps0_fseq l n <ε₀ eps0_fseq l m.
-Proof.
-  induction l using eps0_fseq_rect; intros n m Hnm.
-  + rewrite !eps0_fseq_fix_0; auto.
-    apply eps0_add_mono_right, eps0_exp_S_mono_right; auto.
-  + rewrite !eps0_fseq_fix_1 with (l' := l1); auto.
-    apply eps0_add_mono_right, eps0_omega_mono_lt; auto.
-Qed.
-
-#[local] Hint Resolve eps0_le_refl eps0_lt_le_weak : core.
-
-Fact eps0_max u v b : u <ε₀ b → v <ε₀ b → { w | u ≤ε₀ w ∧ v ≤ε₀ w ∧ w <ε₀ b }.
-Proof. intros ? ?; destruct (eps0_le_lt_dec u v); eauto. Qed.
+  Hint Resolve eps0_lt_trans eps0_add_incr eps0_add_mono_right : core.
 
   (** Another inversion lemma, but this time
       for the limit of the fundemental sequence
@@ -270,249 +182,292 @@ Proof. intros ? ?; destruct (eps0_le_lt_dec u v); eauto. Qed.
       w.r.t. the fundemental sequence of e 
 
       This has become a nice proof *)
-Theorem eps0_lt_fseq_inv e (l : eps0_is_limit e) f : f <ε₀ e → ∃n, f <ε₀ eps0_fseq l n.
-Proof.
-  (* We capture the fundemental sequence via its inductive spec *)
-  revert f; generalize (eps0_fseq l) (eps0_fseq_spec l).
-  clear l.
-  induction 1 as [ e b Hs | e b r Hr H0 Hs IH ]; intros f H.
-  + (* e is _ + ω^{b+1} *)
-    apply eps0_lt_add_inv_add in H as [ H | (g & -> & H) ]; auto.
-    * exists 0.
-      apply eps0_lt_trans with (1 := H).
-      apply eps0_add_incr; auto.
-    * apply eps0_lt_omega_succ_inv in H as (n & Hn).
-      exists n.
-      apply eps0_add_mono_right; auto.
-  + apply eps0_lt_add_inv_add in H as [ H | (g & -> & H) ]; auto.
-    * exists 0.
-      apply eps0_lt_trans with (1 := H).
-      apply eps0_add_incr, eps0_lt_zero_exp_S.
-    * apply eps0_lt_omega_inv in H as [ -> | (a & n & Ha & H) ].
-      - exists 0.
-        apply eps0_add_mono_right, eps0_lt_zero_exp_S.
-      - apply IH in H as (i & Hi).
-        exists i.
+  Theorem eps0_lt_fseq_inv e (l : eps0_is_limit e) f : f <ε₀ e → ∃n, f <ε₀ eps0_fseq l n.
+  Proof.
+    induction l as [ g e l H | g e l l' He IHe ]
+      in f |- * using eps0_fseq_dep_rect;
+      intros [ Hf | (k & -> & Hk) ]%eps0_lt_add_inv_add.
+   + exists 0; rewrite eps0_fseq_fix_0; eauto.
+   + apply eps0_below_omega_succ_inv in Hk as (n & Hn).
+     exists n; rewrite eps0_fseq_fix_0; auto.
+   + exists 0; rewrite eps0_fseq_fix_1 with (l' := l); eauto.
+   + apply eps0_below_omega_inv in Hk as [ -> | (a & n & Ha & H) ].
+     * exists 0; rewrite eps0_fseq_fix_1 with (l' := l); auto.
+     * apply IHe in H as (i & Hi).
+       exists i; rewrite eps0_fseq_fix_1 with (l' := l); auto.
         apply eps0_add_mono_right.
-        apply eps0_lt_trans with (1 := Ha).
-        now apply eps0_exp_S_mono_left.
-Qed.
+        apply eps0_lt_trans with (1 := Ha); auto.
+        now apply eps0_exp_mono_left.
+  Qed.
 
-(** The fundemental sequence is lesser than its limit *)
-Theorem eps0_fseq_lt e (l : eps0_is_limit e) n : eps0_fseq l n <ε₀ e.
-Proof.
-  generalize (eps0_fseq l) (eps0_fseq_spec l) n; clear n l.
-  induction 1 as [ | g b r Hr IH ].
-  + intros; apply eps0_add_mono_right; auto.
-    apply eps0_exp_S_mono_left, eps0_lt_succ.
-  + intros; apply eps0_add_mono_right, eps0_exp_S_mono_left; auto.
-Qed.
+  (** The fundemental sequence is lesser than its limit *)
+  Theorem eps0_fseq_lt e (l : eps0_is_limit e) n : eps0_fseq l n <ε₀ e.
+  Proof.
+    induction l as [ g e l H | g e l l' He IHe ]
+      in n |- * using eps0_fseq_dep_rect.
+    + rewrite eps0_fseq_fix_0; auto. 
+      apply eps0_add_mono_right, eps0_exp_mono_left, eps0_lt_succ.
+    + rewrite eps0_fseq_fix_1 with (l' := l); auto.
+      apply eps0_add_mono_right, eps0_exp_mono_left; auto.
+  Qed.
 
-Fact eps0_mult_exp_S_is_limit a e n :
+  Fact eps0_fseq_omega_succ e (l : eps0_is_limit ω^(S₀ e)) n :
+    eps0_fseq l n = ω^⟨e,n⟩.
+  Proof.
+    revert l; rewrite <- (eps0_add_zero_left ω^_); intros l.
+    rewrite eps0_fseq_fix_0; auto.
+    now rewrite eps0_add_zero_left.
+  Qed.
+
+  Fact eps0_fseq_omega_is_limit e (l : eps0_is_limit ω^e) (l' : eps0_is_limit e) n :
+    eps0_fseq l n = ω^(eps0_fseq l' n).
+  Proof.
+    revert l; rewrite <- (eps0_add_zero_left ω^_); intros l.
+    rewrite eps0_fseq_fix_1 with (l' := l'); auto.
+    now rewrite eps0_add_zero_left.
+  Qed.
+
+  Fact eps0_fseq_exp_S_one e (l : eps0_is_limit ω^⟨S₀ e,1ₚ⟩) n :
+    eps0_fseq l n = ω^⟨e,n⟩.
+  Proof. apply eps0_fseq_omega_succ. Qed.
+
+  Fact eps0_fseq_exp_S_succ e k (l : eps0_is_limit ω^⟨S₀ e,k +ₚ 1ₚ⟩) n :
+    eps0_fseq l n = ω^⟨S₀ e,k⟩ +₀ ω^⟨e,n⟩.
+  Proof.
+    revert l; rewrite <- eps0_add_exp_omega; intros l.
+    rewrite eps0_fseq_fix_0; auto.
+  Qed.
+
+  Fact eps0_fseq_exp_one_is_limit e (l : eps0_is_limit ω^⟨e,1ₚ⟩) (l' : eps0_is_limit e) n :
+    eps0_fseq l n = ω^(eps0_fseq l' n).
+  Proof. apply eps0_fseq_omega_is_limit. Qed.
+
+  Fact eps0_fseq_exp_succ_is_limit e i (l : eps0_is_limit ω^⟨e,i +ₚ 1ₚ⟩) (l' : eps0_is_limit e) n :
+    eps0_fseq l n = ω^⟨e,i⟩ +₀ ω^(eps0_fseq l' n).
+  Proof.
+    revert l; rewrite <- eps0_add_exp_omega; intros l.
+    rewrite eps0_fseq_fix_1 with (l' := l'); auto.
+  Qed.
+
+  (* Another computation for fseq :
+     fseq (ω^e.i +₀ f) n = ω^e.i + fseq f n when f < ω^e *)
+  Lemma eps0_fseq_hnf e i f (l : eps0_is_limit (ω^⟨e,i⟩ +₀ f)) (l' : eps0_is_limit f) n :
+    f <ε₀ ω^e → eps0_fseq l n = ω^⟨e,i⟩ +₀ eps0_fseq l' n.
+  Proof.
+    intros Hf; revert l.
+    induction l' as [ | g b lb ] using eps0_fseq_dep_rect; rewrite <- eps0_add_assoc; intros l.
+    + rewrite !eps0_fseq_fix_0, eps0_add_assoc; auto.
+    + rewrite !eps0_fseq_fix_1 with (l' := lb), eps0_add_assoc; auto.
+  Qed.
+
+  Hint Resolve eps0_le_refl eps0_lt_le_weak : core.
+
+  Fact eps0_max u v b : u <ε₀ b → v <ε₀ b → { w | u ≤ε₀ w ∧ v ≤ε₀ w ∧ w <ε₀ b }.
+  Proof. intros ? ?; destruct (eps0_le_lt_dec u v); eauto. Qed.
+
+  Fact eps0_mult_exp_is_limit a e n :
     0₀ <ε₀ a → 0₀ <ε₀ e → eps0_is_limit (a *₀ ω^⟨e,n⟩).
-Proof.
-  intros Ha He.
-  destruct a as [ | b i c H1 H2 ] using eps0_head_rect.
-  + contradict Ha; apply eps0_lt_irrefl.
-  + rewrite eps0_mult_head_exp_S; auto.
-    apply eps0_is_limit_exp_S.
-    intros (-> & ->)%eps0_add_eq_zero.
-    revert He; apply eps0_lt_irrefl.
-Qed.
+  Proof.
+    intros Ha He.
+    destruct a as [ | b i c H1 H2 ] using eps0_hnf_rect.
+    + contradict Ha; apply eps0_lt_irrefl.
+    + rewrite eps0_mult_hnf_exp; auto.
+      apply eps0_is_limit_exp.
+      intros (-> & ->)%eps0_add_eq_zero.
+      revert He; apply eps0_lt_irrefl.
+  Qed.
 
-(* Of course, if a is 0 then a*e = 0 is not a limit ordinal
-   is the sense we use for the fundemental sequence *)
-Fact eps0_mult_is_limit a e :
+  Hint Resolve eps0_is_succ_exp_zero : core.
+
+  (* Of course, if a is 0 then a*e = 0 is not a limit ordinal
+     is the sense we use for the fundemental sequence *)
+  Fact eps0_mult_is_limit a e :
     0₀ <ε₀ a → eps0_is_limit e → eps0_is_limit (a *₀ e).
-Proof.
-  intros Ha.
-  induction e as [ | | e n f He Hf IHe IHf ] using eps0_head_pos_rect.
-  + now rewrite eps0_mult_zero_right.
-  + intros [H1 H2].
-    destruct H2; auto.
-  + intros [ (-> & H) | H ]%eps0_add_is_limit_inv.
-    * rewrite eps0_add_zero_right; apply eps0_mult_exp_S_is_limit; auto.
-    * rewrite eps0_mult_distr.
-      apply eps0_add_is_limit; auto.
-Qed.
+  Proof.
+    intros Ha.
+    induction e as [ | | e n f He Hf IHe IHf ] using eps0_hnf_pos_rect.
+    + now rewrite eps0_mult_zero_right.
+    + intros [_ []]; auto.
+    + intros [ (-> & H) | H ]%eps0_add_is_limit_inv.
+      * rewrite eps0_add_zero_right; apply eps0_mult_exp_is_limit; auto.
+      * rewrite eps0_mult_distr; apply eps0_add_is_limit; auto.
+  Qed.
 
-Fact eps0_mult_head_limit a i b e :
+  Fact eps0_mult_hnf_limit a i b e :
       b <ε₀ ω^a
     → eps0_is_limit e
     → (ω^⟨a,i⟩ +₀ b) *₀ e = ω^a *₀ e.
-Proof.
-  intros Hab.
-  induction e as [ | e n f H _ IHf ] using eps0_head_rect.
-  + now intros [ [] _ ].
-  + intros He.
-    unfold eps0_omega.
-    assert (e ≠ 0₀) as He'.
-    1:{ intros ->.
-        rewrite eps0_omega_zero in H.
-        apply eps0_lt_one in H as ->.
-        rewrite eps0_add_zero_right in He.
-        apply (proj2 He); auto. }
-    assert (0₀ <ε₀ e) as He''.
-    1:{ now destruct (eps0_zero_or_pos e) as [ -> | ]. }
-    apply eps0_add_is_limit_inv in He as [ (-> & _) | Hf ].
-    * rewrite !eps0_add_zero_right, eps0_mult_head_exp_S, eps0_mult_exp_S; auto.
-    * rewrite eps0_mult_head, IHf, eps0_mult_exp_S_head; auto.
-Qed.
+  Proof.
+    intros Hab.
+    induction e as [ | e n f H _ IHf ] using eps0_hnf_rect.
+    + now intros [ [] _ ].
+    + intros He.
+      unfold eps0_omega.
+      assert (e ≠ 0₀) as He'.
+      1:{ intros ->.
+          rewrite eps0_omega_zero in H.
+          apply eps0_lt_one in H as ->.
+          rewrite eps0_add_zero_right in He.
+          apply (proj2 He); auto. }
+      assert (0₀ <ε₀ e) as He''.
+      1:{ now destruct (eps0_zero_or_pos e) as [ -> | ]. }
+      apply eps0_add_is_limit_inv in He as [ (-> & _) | Hf ].
+      * rewrite !eps0_add_zero_right, eps0_mult_hnf_exp, eps0_mult_exp; auto.
+      * rewrite eps0_mult_hnf, IHf, eps0_mult_exp_hnf; auto.
+  Qed.
 
-#[local] Hint Resolve eps0_add_incr_left 
+  Hint Resolve eps0_add_incr_left 
      eps0_add_incr_right 
      eps0_lt_succ 
      eps0_add_is_limit eps0_is_limit_omega
      eps0_add_mono eps0_add_mono_right : core.
 
+  (** Notice that there are examples where fseq (a+e) n < a + fseq e n
+      for instance a = ω³+ω and e = ω²
 
-(** Notice that there are examples where fseq (a+e) n < a + fseq e n
-    for instance a = ω³+ω and e = ω²
+      a+e = ω³+ω+ω² = ω³+ω²
+      fseq e n = fseq ω² n = ω.(n+1)
+      fseq (a+e) n = fseq (ω³+ω²) n = ω³+ω.(n+1)
+      a+(fseq e n) = ω³+ω+ω.(n+1) = ω³+ω.(n+2)
+      and hence fseq (a+e) n < fseq (a+e) n + ω = a+(fseq e n) *)
 
-    a+e = ω³+ω+ω² = ω³+ω²
-    fseq e n = fseq ω² n = ω.(n+1)
-    fseq (a+e) n = fseq (ω³+ω²) n = ω³+ω.(n+1)
-    a+(fseq e n) = ω³+ω+ω.(n+1) = ω³+ω.(n+2)
-    and hence fseq (a+e) n < fseq (a+e) n + ω = a+(fseq e n) *) 
-Theorem eps0_fseq_add a e (le : eps0_is_limit e) (lae : eps0_is_limit (a+₀e)) :
-   ∀n, eps0_fseq lae n ≤ε₀ a +₀ eps0_fseq le n.
-Proof.
-  revert e le lae.
-  induction a as [ | b i c Hc _ IH ] using eps0_head_rect.
-  + intro e; rewrite (eps0_add_zero_left e).
-    intros; rewrite eps0_add_zero_left; auto.
-    right; apply eps0_fseq_pirr.
-  + intros e; destruct e as [ | f n g Hg _ _ ] using eps0_head_rect.
+  Theorem eps0_fseq_add a e (le : eps0_is_limit e) (lae : eps0_is_limit (a+₀e)) :
+     ∀n, eps0_fseq lae n ≤ε₀ a +₀ eps0_fseq le n.
+  Proof.
+    revert e le lae.
+    induction a as [ | b i c Hc _ IH ] using eps0_hnf_rect.
+    + intro e; rewrite (eps0_add_zero_left e).
+      intros; rewrite eps0_add_zero_left; auto.
+      right; apply eps0_fseq_pirr.
+    + intros e; destruct e as [ | f n g Hg _ _ ] using eps0_hnf_rect.
+      1: intros l; exfalso; now apply (proj1 l).
+      intros le.
+      destruct (eps0_lt_sdec b f) as [ b f Hbf | f | b f Hbf ].
+      * rewrite eps0_add_hnf_lt; auto.
+        intros lae j.
+        rewrite (eps0_fseq_pirr le lae); auto.
+      * rewrite eps0_add_hnf_eq; auto.
+        generalize le.
+        apply eps0_add_is_limit_iff in le
+          as [ (-> & Hf%eps0_is_limit_exp_iff) | Hg' ].
+        - rewrite !eps0_add_zero_right.
+          destruct (pos_add_is_succ i n) as (k & Hk).
+          rewrite Hk.
+          intros le lae m.
+          destruct f as [ | f | f Hf' ] using eps0_discriminate.
+          ++ easy.
+          ++ rewrite eps0_fseq_exp_S_succ.
+             destruct (pos_one_or_succ n) as [ -> | (z & ->) ].
+             ** apply pos_succ_inj in Hk as <-.
+                rewrite eps0_fseq_exp_S_one; auto.
+             ** rewrite <- pos_add_assoc in Hk.
+                apply pos_succ_inj in Hk as <-.
+                rewrite eps0_fseq_exp_S_succ, eps0_add_hnf_eq; auto.
+                apply eps0_exp_mono_left; auto.
+          ++ rewrite eps0_fseq_exp_succ_is_limit with (l' := Hf').
+             destruct (pos_one_or_succ n) as [ -> | (z & ->) ].
+             ** apply pos_succ_inj in Hk as <-.
+                rewrite eps0_fseq_exp_one_is_limit with (l' := Hf'); auto.
+             ** rewrite <- pos_add_assoc in Hk.
+                apply pos_succ_inj in Hk as <-.
+                rewrite <- eps0_add_exp,
+                           eps0_fseq_exp_succ_is_limit with (l' := Hf'),
+                          !eps0_add_assoc; auto.
+        - intros le lae m.
+          rewrite !eps0_fseq_hnf with (l' := Hg'); auto.
+          rewrite <- eps0_add_exp, !eps0_add_assoc; auto.
+      * rewrite eps0_add_assoc.
+        intros lae m.
+        generalize (eps0_add_is_limit_inv _ _ le); intros [ (-> & Hf) | Hg' ].
+        - revert le lae; rewrite !eps0_add_zero_right; intros le lae.
+          assert (eps0_is_limit (c+₀ω^⟨f,n⟩)) as l' by auto.
+          rewrite eps0_fseq_hnf with (l' := l'), eps0_add_assoc; auto.
+          apply eps0_add_below_omega; auto; apply eps0_exp_mono_left; auto.
+        - revert lae; rewrite <- (eps0_add_assoc c); intros lae.
+          assert (eps0_is_limit (c+₀ω^⟨f,n⟩+₀g)) as l' by auto.
+          rewrite eps0_fseq_hnf with (l' := l'); auto.
+          ++ rewrite eps0_add_assoc.
+             apply eps0_add_mono; auto.
+             revert l'; rewrite eps0_add_assoc; auto.
+          ++ apply eps0_add_below_omega.
+             ** apply eps0_add_below_omega; auto.
+                apply eps0_exp_mono_left; auto.
+             ** now apply eps0_lt_trans with (1 := Hg), eps0_omega_mono_lt.
+  Qed.
+
+  Hint Resolve eps0_zero_lt_succ eps0_is_limit_pos : core.
+
+  (** We start with fseq (ω^a * e) *)
+  Lemma eps0_fseq_mult_omega a e (le : eps0_is_limit e) (lae : eps0_is_limit (ω^a*₀e)) :
+     ∀n, eps0_fseq lae n ≤ε₀ ω^a *₀ eps0_fseq le n.
+  Proof.
+    revert le lae.
+    induction e as [ | f n g H IHf IHg ] using eps0_hnf_rect.
     1: intros l; exfalso; now apply (proj1 l).
-    intros le.
-    destruct (eps0_lt_sdec b f) as [ b f Hbf | f | b f Hbf ].
-    * rewrite eps0_add_head_lt; auto.
-      intros lae j.
-      rewrite (eps0_fseq_pirr le lae); auto.
-    * rewrite eps0_add_head_eq; auto.
-      generalize le.
-      apply eps0_add_is_limit_iff in le
-        as [ (-> & Hf%eps0_is_limit_exp_S_iff) | Hg' ].
-      - rewrite !eps0_add_zero_right.
-        destruct (pos_add_is_succ i n) as (k & Hk).
-        rewrite Hk.
-        intros le lae m.
-        destruct f as [ | f | f Hf' ] using eps0_discriminate.
-        ++ easy.
-        ++ rewrite eps0_fseq_exp_S_succ_succ.
-           destruct (pos_one_or_succ n) as [ -> | (z & ->) ].
-           ** apply pos_succ_inj in Hk as <-.
-              rewrite eps0_fseq_exp_S_succ_one; auto.
-           ** rewrite <- pos_add_assoc in Hk.
-              apply pos_succ_inj in Hk as <-.
-              rewrite eps0_fseq_exp_S_succ_succ, eps0_add_head_eq; auto.
-              apply eps0_exp_S_mono_left; auto.
-        ++ rewrite eps0_fseq_exp_S_succ_is_limit with (l' := Hf').
-           destruct (pos_one_or_succ n) as [ -> | (z & ->) ].
-           ** apply pos_succ_inj in Hk as <-.
-              rewrite eps0_fseq_exp_S_one_is_limit with (l' := Hf'); auto.
-           ** rewrite <- pos_add_assoc in Hk.
-              apply pos_succ_inj in Hk as <-.
-              rewrite <- eps0_add_exp_S,
-                         eps0_fseq_exp_S_succ_is_limit with (l' := Hf'),
-                        !eps0_add_assoc; auto.
-      - intros le lae m.
-        rewrite !eps0_fseq_head with (l' := Hg'); auto.
-        rewrite <- eps0_add_exp_S, !eps0_add_assoc; auto.
-    * rewrite  eps0_add_assoc.
-      intros lae m.
-      generalize (eps0_add_is_limit_inv _ _ le); intros [ (-> & Hf) | Hg' ].
-      - revert le lae; rewrite !eps0_add_zero_right; intros le lae.
-        assert (eps0_is_limit (c+₀ω^⟨f,n⟩)) as l' by auto.
-        rewrite eps0_fseq_head with (l' := l'), eps0_add_assoc; auto.
-        apply eps0_add_below_omega; auto; apply eps0_exp_S_mono_left; auto.
-      - revert lae; rewrite <- (eps0_add_assoc c); intros lae.
-        assert (eps0_is_limit (c+₀ω^⟨f,n⟩+₀g)) as l' by auto.
-        rewrite eps0_fseq_head with (l' := l'); auto.
-        ++ rewrite eps0_add_assoc.
-           apply eps0_add_mono; auto.
-           revert l'; rewrite eps0_add_assoc; auto.
-        ++ apply eps0_add_below_omega.
-           ** apply eps0_add_below_omega; auto.
-              apply eps0_exp_S_mono_left; auto.
-           ** now apply eps0_lt_trans with (1 := Hg), eps0_omega_mono_lt.
-Qed.
+    destruct f as [ | f | f Hf ] using eps0_discriminate.
+    + rewrite eps0_omega_zero in H.
+      apply eps0_lt_one in H as ->.
+      rewrite eps0_add_zero_right; auto.
+      intros le; exfalso; apply (proj2 le); auto.
+    + rewrite eps0_mult_omega_hnf; auto.
+      intros le lae i.
+      generalize (eps0_add_is_limit_inv _ _ le); intros [ (-> & Hf) | Hg ].
+      * revert le lae. 
+        rewrite eps0_mult_zero_right, !eps0_add_zero_right, eps0_add_succ_right.
+        intros le lae.
+        destruct (pos_one_or_succ n) as [ -> | (m & ->) ].
+        - rewrite !eps0_fseq_exp_S_one, eps0_mult_omega_exp; auto.
+        - rewrite !eps0_fseq_exp_S_succ, eps0_mult_distr, 
+                  !eps0_mult_omega_exp, eps0_add_succ_right; auto.
+      * assert (eps0_is_limit (ω^(a) *₀ g)) as Hag.
+        1: apply eps0_mult_is_limit; auto.
+        rewrite eps0_fseq_hnf with (l' := Hg); auto.
+        rewrite eps0_fseq_hnf with (l' := Hag); auto.
+        - rewrite eps0_mult_distr, eps0_mult_omega_exp; auto.
+        - apply eps0_mult_below_omega with (n := 1); auto.
+          apply eps0_exp_mono_right; auto.
+    + rewrite eps0_mult_omega_hnf; auto.
+      intros le lae i.
+      generalize (eps0_add_is_limit_inv _ _ le); intros [ (-> & Hf') | Hg ].
+      * revert le lae.
+        rewrite eps0_mult_zero_right, !eps0_add_zero_right.
+        intros le lae.
+        assert (eps0_is_limit (a +₀ f)) as Haf by auto.
+        destruct (pos_one_or_succ n) as [ -> | (m & ->) ].
+        - rewrite eps0_fseq_exp_one_is_limit with (l' := Hf),
+                  eps0_fseq_exp_one_is_limit with (l' := Haf),
+                  eps0_mult_omega. 
+          apply eps0_omega_mono_le, eps0_fseq_add.
+        - rewrite eps0_fseq_exp_succ_is_limit with (l' := Hf),
+                  eps0_fseq_exp_succ_is_limit with (l' := Haf),
+                  eps0_mult_distr, eps0_mult_omega_exp, 
+                  eps0_mult_omega.
+          apply eps0_add_mono; auto.
+          apply eps0_omega_mono_le, eps0_fseq_add.
+      * assert (eps0_is_limit (ω^(a) *₀ g)) as Hag.
+        1: apply eps0_mult_is_limit; auto.
+        rewrite eps0_fseq_hnf with (l' := Hg); auto.
+        rewrite eps0_fseq_hnf with (l' := Hag); auto.
+        - rewrite eps0_mult_distr, eps0_mult_omega_exp; auto.
+        - apply eps0_mult_below_omega with (n := 1); auto.
+          apply eps0_exp_mono_right; auto.
+  Qed.
 
-Hint Resolve eps0_zero_lt_succ : core.
+  Theorem eps0_fseq_mult a e (le : eps0_is_limit e) (lae : eps0_is_limit (a*₀e)) :
+     ∀n, eps0_fseq lae n ≤ε₀ a *₀ eps0_fseq le n.
+  Proof.
+    destruct a as [ | a i b Hb _ _ ] using eps0_hnf_rect.
+    + exfalso.
+      rewrite eps0_mult_zero_left in lae.
+      now apply (proj1 lae).
+    + revert lae.
+      rewrite eps0_mult_hnf_limit; auto.
+      intros lae n.
+      apply eps0_le_trans with (1 := eps0_fseq_mult_omega _ le lae n).
+      apply eps0_mult_mono; auto.
+      apply eps0_le_trans with ω^⟨a,i⟩; auto.
+      apply eps0_exp_mono; auto.
+  Qed.
 
-(** We start with fseq (ω^a * e) *)
-Lemma eps0_fseq_mult_omega a e (le : eps0_is_limit e) (lae : eps0_is_limit (ω^a*₀e)) :
-   ∀n, eps0_fseq lae n ≤ε₀ ω^a *₀ eps0_fseq le n.
-Proof.
-  revert le lae.
-  destruct e as [ | f n g H IHf IHg ] using eps0_head_rect.
-  1: intros l; exfalso; now apply (proj1 l).
-  destruct f as [ | f | f Hf ] using eps0_discriminate.
-  + rewrite eps0_omega_zero in H.
-    apply eps0_lt_one in H as ->.
-    rewrite eps0_add_zero_right; auto.
-    intros le; exfalso; apply (proj2 le); auto.
-  + rewrite eps0_mult_omega_head; auto.
-    intros le lae i.
-    generalize (eps0_add_is_limit_inv _ _ le); intros [ (-> & Hf) | Hg ].
-    * revert le lae. 
-      rewrite eps0_mult_zero_right, !eps0_add_zero_right, eps0_add_succ_right.
-      intros le lae.
-      destruct (pos_one_or_succ n) as [ -> | (m & ->) ].
-      - rewrite !eps0_fseq_exp_S_succ_one, eps0_mult_omega_exp_S; auto.
-      - rewrite !eps0_fseq_exp_S_succ_succ, eps0_mult_distr, 
-                !eps0_mult_omega_exp_S, eps0_add_succ_right; auto.
-    * assert (eps0_is_limit (ω^(a) *₀ g)) as Hag.
-      1:{ apply eps0_mult_is_limit; auto. }
-      rewrite eps0_fseq_head with (l' := Hg); auto.
-      rewrite eps0_fseq_head with (l' := Hag); auto.
-      - rewrite eps0_mult_distr, eps0_mult_omega_exp_S.
-        apply eps0_add_mono; auto.
-      - apply eps0_mult_below_omega with (n := 1); auto.
-        apply eps0_exp_S_mono_right; auto.
-  + rewrite eps0_mult_omega_head; auto.
-    intros le lae i.
-    generalize (eps0_add_is_limit_inv _ _ le); intros [ (-> & Hf') | Hg ].
-    * revert le lae.
-      rewrite eps0_mult_zero_right, !eps0_add_zero_right.
-      intros le lae.
-      assert (eps0_is_limit (a +₀ f)) as Haf by auto.
-      destruct (pos_one_or_succ n) as [ -> | (m & ->) ].
-      - rewrite eps0_fseq_exp_S_one_is_limit with (l' := Hf),
-                eps0_fseq_exp_S_one_is_limit with (l' := Haf),
-                eps0_mult_omega. 
-        apply eps0_omega_mono_le, eps0_fseq_add.
-      - rewrite eps0_fseq_exp_S_succ_is_limit with (l' := Hf),
-                eps0_fseq_exp_S_succ_is_limit with (l' := Haf),
-                eps0_mult_distr, eps0_mult_omega_exp_S, 
-                eps0_mult_omega.
-        apply eps0_add_mono; auto.
-        apply eps0_omega_mono_le, eps0_fseq_add.
-    * assert (eps0_is_limit (ω^(a) *₀ g)) as Hag.
-      1:{ apply eps0_mult_is_limit; auto. }
-      rewrite eps0_fseq_head with (l' := Hg); auto.
-      rewrite eps0_fseq_head with (l' := Hag); auto.
-      - rewrite eps0_mult_distr, eps0_mult_omega_exp_S.
-        apply eps0_add_mono; auto.
-      - apply eps0_mult_below_omega with (n := 1); auto.
-        apply eps0_exp_S_mono_right; auto.
-Qed.
-
-Theorem eps0_fseq_mult a e (le : eps0_is_limit e) (lae : eps0_is_limit (a*₀e)) :
-   ∀n, eps0_fseq lae n ≤ε₀ a *₀ eps0_fseq le n.
-Proof.
-  destruct a as [ | a i b Hb _ _ ] using eps0_head_rect.
-  + exfalso.
-    rewrite eps0_mult_zero_left in lae.
-    now apply (proj1 lae).
-  + revert lae.
-    rewrite eps0_mult_head_limit; auto.
-    intros lae n.
-    apply eps0_le_trans with (1 := eps0_fseq_mult_omega _ le lae n).
-    apply eps0_mult_mono; auto.
-    apply eps0_le_trans with ω^⟨a,i⟩; auto.
-    apply eps0_exp_S_mono; auto.
-    apply pos_one_least.
-Qed.
-
+End eps0_fseq.
 
