theories/eps0_ltf.v
@@ -1,0 +1,170 @@
+(**************************************************************)
+(*   Copyright Dominique Larchey-Wendling [*]                 *)
+(*                                                            *)
+(*                             [*] Affiliation LORIA -- CNRS  *)
+(**************************************************************)
+(*      This file is distributed under the terms of the       *)
+(*        Mozilla Public License Version 2.0, MPL-2.0         *)
+(**************************************************************)
+
+From Coq Require Import List Relations Arith Lia Wellfounded Utf8.
+From Hydra Require Import utils pos eps0.
+
+Import ListNotations.
+
+Set Implicit Arguments.
+
+(** The least tail form (ltf) of an ordinal is a decomposition
+    of the form a + ω^e for with a is the least possible 
+ 
+    Hence for instance:
+     - 0 + ω is a ltf
+     - ω³ + ω is a ltf
+     - but (ω³+ω) + ω² is not a ltf  *)
+
+Definition eps0_ltf a e := ∀b, a +₀ ω^e = b +₀ ω^e → a ≤ε₀ b.
+
+#[local] Hint Resolve eps0_zero_least : core.
+
+#[local] Hint Resolve eps0_le_antisym : core.
+
+#[local] Hint Resolve eps0_le_refl eps0_le_trans eps0_lt_trans 
+                      eps0_lt_le_weak : core.
+
+#[local] Hint Resolve eps0_add_mono eps0_add_incr 
+                      eps0_add_incr_left eps0_add_incr_right : core.
+
+Fact eps0_ltf_zero e : eps0_ltf 0₀ e.
+Proof. red; auto. Qed.
+
+Fact eps0_eq_ltf_inv :
+  ∀ a b e f,
+      eps0_ltf a e
+    → eps0_ltf b f
+    → a +₀ ω^e = b +₀ ω^f
+    → a = b ∧ e = f.
+Proof.
+  intros a b e f H1 H2 E.
+  assert (e = f) as <-; auto.
+  1: now apply eps0_tf_fun_right in E.
+Qed.
+
+#[local] Hint Resolve eps0_ltf_zero : core. 
+
+Fact eps0_one_eq_ltf a e :
+    eps0_ltf a e
+  → 1₀ = a +₀ ω^e
+  → a = 0₀ ∧ e = 0₀.
+Proof.
+  intros H1.
+  replace 1₀ with (0₀ +₀ ω^0₀).
+  + intros (<- & <-)%eps0_eq_ltf_inv; eauto.
+  + now rewrite eps0_add_zero_left, eps0_omega_zero.
+Qed.
+
+Fact eps0_eq_omega_ltf_inv a b e :
+    eps0_ltf b e
+  → ω^a = b +₀ ω^e
+  → b = 0₀ ∧ a = e.
+Proof.
+  intros H.
+  rewrite <- (eps0_add_zero_left ω^a).
+  intros (<- & <-)%eps0_eq_ltf_inv; auto.
+Qed.
+
+Fact eps0_ltf_exp e n : eps0_ltf ω^⟨e,n⟩ e.
+Proof.
+  intros b Hb.
+  rewrite eps0_add_exp_omega in Hb.
+  destruct b as [ | g i f Hf _ ] using eps0_hnf_rect.
+  + rewrite eps0_add_zero_left in Hb.
+    now apply eps0_exp_inj, proj2, pos_succ_neq_one in Hb.
+  + rewrite <- (eps0_add_zero_right ω^e) in Hb; unfold eps0_omega in Hb.
+    destruct (eps0_lt_sdec g e) as [ g e C | e | g e C ].
+    * rewrite eps0_add_hnf_lt, eps0_add_zero_right in Hb; auto.
+      now apply eps0_exp_inj, proj2, pos_succ_neq_one in Hb.
+    * rewrite eps0_add_hnf_eq, eps0_add_zero_right in Hb; auto.
+      apply eps0_exp_inj, proj2, pos_succ_inj in Hb as <-; auto.
+    * apply eps0_le_trans with ω^⟨g,i⟩; auto.
+      left; now apply eps0_exp_mono_left.
+Qed.
+
+Fact eps0_ltf_hnf e n g h : 
+    g +₀ ω^(h) <ε₀ ω^(e)
+  → eps0_ltf g h
+  → eps0_ltf (ω^⟨e,n⟩ +₀ g) h.
+Proof.
+  intros Hg Hgh b Hb.
+  destruct (eps0_le_lt_dec (ω^⟨e,n⟩ +₀ g) b) as [ | [C | (b' & -> & Hb2)]%eps0_lt_add_inv_add ]; auto.
+  + assert (ω^h <ε₀ ω^e) as Hh. 
+    1:{ apply eps0_le_lt_trans with (2 := Hg); auto. }
+    destruct (@eps0_lt_irrefl ω^⟨e,n⟩).
+    apply eps0_le_lt_trans with (2 := eps0_add_below_exp _ _ C Hh).
+    rewrite <- Hb, eps0_add_assoc; auto.
+  + apply eps0_add_mono; auto.
+    apply Hgh.
+    rewrite !eps0_add_assoc in Hb.
+    apply eps0_eq_hnf_inv in Hb as (_ & _ & Hb); auto.
+    apply eps0_le_lt_trans with (2 := Hg); auto.
+Qed.
+
+Fact eps0_ltf_hnf' e g i f :
+      g <ε₀ ω^e
+    → ω^f <ε₀ ω^e
+    → eps0_ltf g f
+    → eps0_ltf (ω^⟨e,i⟩ +₀ g) f.
+Proof. intros ? ?; apply eps0_ltf_hnf, eps0_add_below_omega; auto. Qed.
+
+Section eps0_ltf_rect.
+
+  Inductive eps0_ltf_decomp : ε₀ → Type :=
+    | eps0_ld_zero :    eps0_ltf_decomp 0₀
+    | eps0_ld_ltf g e : eps0_ltf g e
+                      → eps0_ltf_decomp (g +₀ ω^e).
+
+  Hint Constructors eps0_ltf_decomp : core.
+  Hint Resolve eps0_ltf_exp eps0_ltf_hnf : core.
+
+  Local Fact eps0_ld_exp e n : eps0_ltf_decomp ω^⟨e,n⟩.
+  Proof.
+    destruct (pos_one_or_succ n) as [ -> | (m & ->) ].
+    + rewrite <- eps0_add_zero_left; constructor 2; auto.
+    + rewrite <- eps0_add_exp_omega; eauto.
+  Qed.
+
+  Hint Resolve eps0_ld_exp : core.
+
+  Lemma eps0_ld_build e : eps0_ltf_decomp e.
+  Proof.
+    induction e as [ | e n f H _ IH ] using eps0_hnf_rect; auto.
+    destruct IH as [ | g h IH ].
+    + rewrite eps0_add_zero_right; auto.
+    + rewrite <- eps0_add_assoc; auto.
+  Qed.
+
+  Section eps0_ltf_rect.
+
+    (** Induction principle corresponding to the following building rules 
+        for ordinals below ε₀:
+
+                       g  e  eps0_ltf g e
+            ------   ----------------------
+              0₀          g +₀ ω^e
+     *)
+
+    Variables (P : ε₀ → Type)
+            (HP0 : P 0₀)
+            (HP2 : ∀ g e, eps0_ltf g e → P g → P e → P (g +₀ ω^e)).
+
+    Hint Resolve eps0_lt_le_trans eps0_lt_omega : core.
+
+    Theorem eps0_ltf_rect e : P e.
+    Proof.
+      induction e as [ e IH ] using eps0_rect.
+      destruct (eps0_ld_build e); auto.
+      apply HP2; eauto.
+    Qed.
+
+  End eps0_ltf_rect.
+
+End eps0_ltf_rect.
