theories/eps0_mult.v
@@ -1,0 +1,781 @@
+(**************************************************************)
+(*   Copyright Dominique Larchey-Wendling [*]                 *)
+(*                                                            *)
+(*                             [*] Affiliation LORIA -- CNRS  *)
+(**************************************************************)
+(*      This file is distributed under the terms of the       *)
+(*        Mozilla Public License Version 2.0, MPL-2.0         *)
+(**************************************************************)
+
+From Coq Require Import List Relations Arith Lia Wellfounded Utf8.
+From Hydra Require Import utils pos ordered eps0.
+
+Import ListNotations.
+
+Set Implicit Arguments.
+
+#[local] Notation π₁ := proj1_sig.
+#[local] Notation π₂ := proj2_sig.
+
+#[local] Hint Resolve eps0_le_refl eps0_lt_succ
+                      eps0_zero_least
+                      eps0_add_incr
+                      eps0_add_mono_right
+                      eps0_lt_zero_exp 
+                      eps0_zero_lt_omega 
+                      eps0_lt_le_weak 
+                      eps0_add_mono_left 
+                      eps0_add_mono
+                      eps0_add_incr_left
+                      eps0_add_incr_right
+: core.
+
+Section eps0_mpos.
+
+  (** pos := nat viewed as 1, 2, ... and not 0, 1, ... *)
+
+  (** The operation (θ : ε₀) (n : pos) => θ.(1+n) *)
+  Inductive eps0_mpos_gr n : ε₀ → ε₀ → Prop :=
+    | eps0_mpos_gr_0 : eps0_mpos_gr n 0₀ 0₀
+    | eps0_mpos_gr_1 α i β : β <ε₀ ω^α → eps0_mpos_gr n (ω^⟨α,i⟩ +₀ β) (ω^⟨α,i *ₚ n⟩ +₀ β).
+
+  Fact eps0_mpos_fun n e1 f1 e2 f2 : eps0_mpos_gr n e1 f1 → eps0_mpos_gr n e2 f2 → e1 = e2 → f1 = f2.
+  Proof.
+    do 2 destruct 1; auto.
+    + now intros ?%eps0_zero_neq_hnf.
+    + symm; now intros ?%eps0_zero_neq_hnf.
+    + intros (? & [])%eps0_eq_hnf_inv; subst; auto.
+  Qed.
+
+  Definition eps0_mpos_pwc e n : sig (eps0_mpos_gr n e).
+  Proof.
+    destruct e as [ | e i f ] using eps0_hnf_rect.
+    + exists 0₀; constructor.
+    + exists (ω^⟨e,i *ₚ n⟩ +₀ f); now constructor.
+  Qed.
+
+  Definition eps0_mpos e n := π₁ (eps0_mpos_pwc e n).
+
+  Fact eps0_mpos_spec e n : eps0_mpos_gr n e (eps0_mpos e n).
+  Proof. apply (proj2_sig _). Qed.
+
+  Fact eps0_mpos_fix_0 n : eps0_mpos 0₀ n = 0₀.
+  Proof. apply eps0_mpos_fun with (1 := eps0_mpos_spec _ _) (3 := eq_refl); constructor. Qed.
+
+  Fact eps0_mpos_fix_1 n α i β : β <ε₀ ω^α → eps0_mpos (ω^⟨α,i⟩ +₀ β) n = ω^⟨α,i *ₚ n⟩ +₀ β.
+  Proof. intros; apply eps0_mpos_fun with (1 := eps0_mpos_spec _ _) (3 := eq_refl); now constructor. Qed.
+
+  Fact eps0_mpos_exp n α i : eps0_mpos ω^⟨α,i⟩ n = ω^⟨α,i *ₚ n⟩.
+  Proof. 
+    rewrite <- (eps0_add_zero_right ω^⟨_,i⟩), eps0_mpos_fix_1; auto.
+    now rewrite eps0_add_zero_right.
+  Qed.
+
+  Fact eps0_mpos_one e : eps0_mpos e 1ₚ = e.
+  Proof.
+    destruct e using eps0_hnf_rect.
+    + now rewrite eps0_mpos_fix_0.
+    + rewrite eps0_mpos_fix_1, pos_mul_one_right; auto.
+  Qed.
+
+  Fact eps0_mpos_omega_add n α β : β <ε₀ ω^α → eps0_mpos (ω^α +₀ β) n = ω^⟨α,n⟩ +₀ β.
+  Proof.
+    intros; unfold eps0_omega.
+    rewrite eps0_mpos_fix_1; auto.
+  Qed.
+
+  Fact eps0_mpos_omega n α : eps0_mpos ω^α n = ω^⟨α,n⟩.
+  Proof.
+    rewrite <- (eps0_add_zero_right ω^α), eps0_mpos_omega_add; auto.
+    now rewrite eps0_add_zero_right.
+  Qed.
+
+  Fact eps0_mpos_add e i j : eps0_mpos e i +₀ eps0_mpos e j = eps0_mpos e (i +ₚ j).
+  Proof.
+    destruct e using eps0_hnf_rect.
+    + now rewrite !eps0_mpos_fix_0, eps0_add_zero_left.
+    + rewrite !eps0_mpos_fix_1; auto.
+      rewrite eps0_add_hnf_eq, pos_mul_distr_right; auto.
+  Qed.
+
+  Fact eps0_mpos_comp e i j : eps0_mpos (eps0_mpos e i) j = eps0_mpos e (i *ₚ j).
+  Proof.
+    destruct e using eps0_hnf_rect.
+    + now rewrite !eps0_mpos_fix_0.
+    + rewrite !eps0_mpos_fix_1, pos_mul_assoc; auto.
+  Qed.
+
+  Fact eps0_mpos_mono_left a b m n : a <ε₀ b → m ≤ n → eps0_mpos a m <ε₀ eps0_mpos b n.
+  Proof.
+    intros Hab Hmn.
+    destruct a as [ | e i f H1 _ _ ] using eps0_hnf_rect;
+      destruct b as [ | g j h H2 _ _ ] using eps0_hnf_rect.
+    + now apply eps0_lt_irrefl in Hab.
+    + rewrite eps0_mpos_fix_0, eps0_mpos_fix_1; auto.
+    + now apply eps0_zero_not_gt in Hab.
+    + apply eps0_lt_hnf_inv in Hab; auto.
+      rewrite !eps0_mpos_fix_1; auto.
+      apply eps0_lt_hnf_inv; auto.
+      destruct Hab as [ | (<- & [ | (<- & ?) ]) ]; auto.
+      * right; split; auto; left.
+        now apply pos_mul_mono_left.
+      * apply pos_le_lt_iff in Hmn as [ -> | Hmn ]; auto.
+        right; split; auto; left.
+        now apply pos_mul_mono_right.
+  Qed.
+
+  Fact eps0_mpos_gt_zero a n : 0₀ <ε₀ a → 0₀ <ε₀ eps0_mpos a n.
+  Proof.
+    intros H.
+    apply eps0_mpos_mono_left with (n := n) (m := n) in H; auto.
+    now rewrite eps0_mpos_fix_0 in H.
+  Qed.
+
+  Hint Resolve eps0_mpos_mono_left eps0_mpos_gt_zero : core.
+
+  Fact eps0_mpos_mono_right a n m : 0₀ <ε₀ a → n < m → eps0_mpos a n <ε₀ eps0_mpos a m.
+  Proof.
+    intros H1 H2.
+    destruct a as [ | e i f H _ _ ] using eps0_hnf_rect.
+    + now apply eps0_lt_irrefl in H1.
+    + rewrite !eps0_mpos_fix_1; auto.
+      apply eps0_lt_hnf_inv; auto.
+      right; split; auto; left.
+      now apply pos_mul_mono_right.
+  Qed.
+
+  Fact eps0_mpos_mono_right_le a n m : n ≤ m → eps0_mpos a n ≤ε₀ eps0_mpos a m.
+  Proof.
+    destruct (eq_nat_dec n m) as [ <- | ]; auto; intro.
+    destruct (eps0_zero_or_pos a) as [ -> | ].
+    + rewrite !eps0_mpos_fix_0; auto.
+    + left; apply eps0_mpos_mono_right; auto; lia.
+  Qed.
+
+  Fact eps0_mpos_mono a b m n : a ≤ε₀ b → m ≤ n → eps0_mpos a m ≤ε₀ eps0_mpos b n.
+  Proof.
+    intros [ H1 | -> ].
+    + left; now apply eps0_mpos_mono_left.
+    + apply eps0_mpos_mono_right_le.
+  Qed.
+
+  Fact eps0_mpos_below_omega a n e : a <ε₀ ω^e → eps0_mpos a n <ε₀ ω^e.
+  Proof.
+    intros [ -> | (f & i & H1 & H2) ]%eps0_below_omega_inv.
+    + rewrite eps0_mpos_fix_0; auto.
+    + apply eps0_mpos_mono_left with (n := n) (m := n) in H1; auto.
+      apply eps0_lt_trans with (1 := H1).
+      rewrite eps0_mpos_exp.
+      apply eps0_lt_exp_inv; auto.
+  Qed.
+
+  Fact eps0_mpos_below_omega' a n e i : a <ε₀ ω^⟨e,i⟩ → eps0_mpos a n <ε₀ ω^(S₀ e).
+  Proof.
+    intros H.
+    apply eps0_mpos_below_omega,
+          eps0_lt_trans with (1 := H),
+          eps0_exp_mono_left; auto.
+  Qed.
+
+End eps0_mpos.
+
+#[local] Hint Resolve eps0_mpos_mono_left eps0_mpos_gt_zero : core.
+
+Section eps0_momega.
+
+  (** now the operation (θ α : ε₀) => θ.ω^α *)
+  Inductive eps0_momega_gr α : ε₀ → ε₀ → Prop :=
+    | eps0_momega_gr_0 : eps0_momega_gr α 0₀ 0₀
+    | eps0_momega_gr_1 γ n β : β <ε₀ ω^γ → eps0_momega_gr α (ω^⟨γ,n⟩ +₀ β) ω^(γ+₀α).
+
+  Fact eps0_momega_fun a e1 f1 e2 f2 : eps0_momega_gr a e1 f1 → eps0_momega_gr a e2 f2 → e1 = e2 → f1 = f2.
+  Proof.
+    do 2 destruct 1; auto.
+    + now intros ?%eps0_zero_neq_hnf.
+    + symm; now intros ?%eps0_zero_neq_hnf.
+    + intros (? & [])%eps0_eq_hnf_inv; subst; auto.
+  Qed.
+
+  Definition eps0_momega_pwc e α : sig (eps0_momega_gr α e).
+  Proof.
+    destruct e as [ | e ] using eps0_hnf_rect.
+    + exists 0₀; constructor.
+    + exists ω^(e+₀α); now constructor.
+  Qed.
+
+  Definition eps0_momega e α := π₁ (eps0_momega_pwc e α).
+
+  Fact eps0_momega_spec e α : eps0_momega_gr α e (eps0_momega e α).
+  Proof. apply (proj2_sig _). Qed.
+
+  Fact eps0_momega_fix_0 α : eps0_momega 0₀ α = 0₀.
+  Proof. apply eps0_momega_fun with (1 := eps0_momega_spec _ _) (3 := eq_refl); constructor. Qed.
+
+  Fact eps0_momega_fix_1 γ n β α : β <ε₀ ω^γ → eps0_momega (ω^⟨γ,n⟩ +₀ β) α = ω^(γ+₀α).
+  Proof. intros; apply eps0_momega_fun with (1 := eps0_momega_spec _ _) (3 := eq_refl); now constructor. Qed.
+
+  Fact eps0_momega_exp γ n α : eps0_momega ω^⟨γ,n⟩ α = ω^(γ+₀α).
+  Proof. rewrite <- (eps0_add_zero_right ω^⟨_,_⟩), eps0_momega_fix_1; auto. Qed.
+
+  Fact eps0_momega_mpos a i e :
+      0₀ <ε₀ e → eps0_momega (eps0_mpos a i) e = eps0_momega a e.
+  Proof.
+    intros He.
+    destruct a using eps0_hnf_rect.
+    + now rewrite eps0_mpos_fix_0.
+    + rewrite eps0_mpos_fix_1; auto.
+      rewrite !eps0_momega_fix_1; auto.
+  Qed.
+
+  Fact eps0_add_mpos_momega n k e f :
+      0₀ <ε₀ f
+    → eps0_mpos e n +₀ eps0_mpos (eps0_momega e f) k
+    = eps0_mpos (eps0_momega e f) k.
+  Proof.
+    intros Hf.
+    destruct e using eps0_hnf_rect.
+    + now rewrite !eps0_mpos_fix_0, eps0_add_zero_left.
+    + rewrite !eps0_mpos_fix_1; auto.
+      rewrite eps0_momega_fix_1; auto.
+      rewrite !eps0_mpos_omega.
+      rewrite <- (eps0_add_zero_right ω^⟨_,k⟩).
+      rewrite eps0_add_hnf_lt; auto.
+  Qed.
+
+  Fact eps0_mpos_add_momega a e f i j :
+      e <ε₀ f
+    → eps0_mpos (eps0_momega a e) i +₀ eps0_mpos (eps0_momega a f) j
+    = eps0_mpos (eps0_momega a f) j.
+  Proof.
+    intros Hef.
+    destruct a using eps0_hnf_rect.
+    + now rewrite !eps0_momega_fix_0, !eps0_mpos_fix_0, eps0_add_zero_left.
+    + rewrite !eps0_momega_fix_1; auto.
+      rewrite !eps0_mpos_omega, eps0_add_exp_lt; auto.
+  Qed.
+
+  Fact eps0_momega_mono_left a b c :
+      a ≤ε₀ b
+    → eps0_momega a c ≤ε₀ eps0_momega b c.
+  Proof.
+    intros [ Hab | <- ]; auto.
+    destruct a as [ | e i f H1 _ _ ] using eps0_hnf_rect;
+      destruct b as [ | g j h H2 _ _ ] using eps0_hnf_rect.
+    + now apply eps0_lt_irrefl in Hab.
+    + rewrite eps0_momega_fix_0, eps0_momega_fix_1; auto.
+    + now apply eps0_zero_not_gt in Hab.
+    + rewrite !eps0_momega_fix_1; auto.
+      apply eps0_lt_hnf_inv in Hab; auto.
+      apply eps0_omega_mono_le.
+      destruct Hab as [ | (<- & _) ]; auto.
+  Qed.
+
+  Fact eps0_momega_mono_right a b c :
+      0₀ <ε₀ a
+    → b <ε₀ c 
+    → eps0_momega a b <ε₀ eps0_momega a c.
+  Proof.
+    intros H ?.
+    destruct a using eps0_hnf_rect.
+    + now apply eps0_lt_irrefl in H.
+    + rewrite !eps0_momega_fix_1; auto.
+      apply eps0_omega_mono_lt; auto.
+  Qed.
+
+  Fact eps0_momega_lt_pos a e :
+      0₀ <ε₀ a
+    → 0₀ <ε₀ e
+    → ω^e ≤ε₀ eps0_momega a e.
+  Proof.
+    intros Ha He.
+    destruct a using eps0_hnf_rect.
+    + now apply eps0_lt_irrefl in Ha.
+    + rewrite eps0_momega_fix_1; auto.
+      apply eps0_omega_mono_le; auto.
+  Qed.
+
+  Fact eps0_lt_mpos_momega a n f :
+      0₀ <ε₀ a
+    → 0₀ <ε₀ f
+    → eps0_mpos a n <ε₀ eps0_momega a f.
+  Proof.
+    intros Ha Hf.
+    destruct a using eps0_hnf_rect.
+    + now apply eps0_lt_irrefl in Ha.
+    + rewrite eps0_mpos_fix_1, eps0_momega_fix_1; auto.
+      apply eps0_lt_hnf_exp_inv; auto.
+  Qed.
+
+  Fact eps0_momega_below_omega a b e f :
+      a <ε₀ ω^e
+    → b <ε₀ f
+    → eps0_momega a b <ε₀ ω^(e +₀ f).
+  Proof.
+    intros [ -> | (g & i & H1 & H2) ]%eps0_below_omega_inv Hb.
+    + rewrite eps0_momega_fix_0; auto.
+    + apply eps0_le_lt_trans with (eps0_momega ω^⟨g,i⟩ b).
+      * apply eps0_momega_mono_left; auto.
+      * rewrite eps0_momega_exp.
+        apply eps0_omega_mono_lt.
+        apply eps0_lt_le_trans with (g +₀ f); auto.
+  Qed.
+
+  Fact eps0_momega_below_exp a b e n f :
+      a <ε₀ ω^⟨e,n⟩
+    → b <ε₀ f
+    → eps0_momega a b <ε₀ ω^(e +₀ f).
+  Proof.
+    intros [ [ -> | (i & c & -> & ? & ?) ] | (g & i & H1 & ?) ]%eps0_below_exp_inv ?.
+    + rewrite eps0_momega_fix_0; auto.
+    + rewrite eps0_momega_fix_1; auto.
+      apply eps0_omega_mono_lt; auto.
+    + apply eps0_lt_le_weak, eps0_momega_mono_left with (c := b) in H1.
+      apply eps0_le_lt_trans with (1 := H1).
+      rewrite eps0_momega_exp; auto.
+      apply eps0_omega_mono_lt.
+      apply eps0_le_lt_trans with (e +₀ b); auto.
+  Qed.
+
+End eps0_momega.
+
+Section eps0_mult.
+
+  (* now the operation (γ α : ε₀) => γ.α *)
+  Inductive eps0_mult_gr γ : ε₀ → ε₀ → Prop :=
+    | eps0_mult_gr_0         : eps0_mult_gr γ 0₀ 0₀ 
+    | eps0_mult_gr_1 n       : eps0_mult_gr γ ω^⟨0₀,n⟩ (eps0_mpos γ n)
+    | eps0_mult_gr_2 α n β r : 0₀ <ε₀ α
+                             → β <ε₀ ω^α
+                             → eps0_mult_gr γ β r
+                             → eps0_mult_gr γ (ω^⟨α,n⟩ +₀ β) (eps0_mpos (eps0_momega γ α) n +₀ r).
+
+  Fact eps0_mult_fun a e1 f1 e2 f2 :
+      eps0_mult_gr a e1 f1
+    → eps0_mult_gr a e2 f2
+    → e1 = e2
+    → f1 = f2.
+  Proof.
+    intros H1; revert H1 e2 f2.
+    induction 1 as [ | n1 | e1 n1 f1 r1 H1 G1 F1 IH1 ];
+      induction 1 as [ | n2 | e2 n2 f2 r2 H2 G2 F2 _ ]; auto.
+    + now intros ?%eps0_zero_neq_exp.
+    + now intros ?%eps0_zero_neq_hnf.
+    + symm; now intros ?%eps0_zero_neq_exp.
+    + now intros (_ & ->)%eps0_exp_inj.
+    + intros (<- & -> & ->)%eps0_eq_exp_hnf_inv; auto.
+      contradict H2; apply eps0_lt_irrefl.
+    + symm; now intros ?%eps0_zero_neq_hnf.
+    + symm; intros (<- & -> & ->)%eps0_eq_exp_hnf_inv; auto.
+      contradict H1; apply eps0_lt_irrefl.
+    + intros (<- & <- & <-)%eps0_eq_hnf_inv; auto.
+      f_equal; eauto.
+  Qed.
+
+  Hint Constructors eps0_mult_gr : core.
+
+  Definition eps0_mult_pwc γ e : sig (eps0_mult_gr γ e).
+  Proof.
+    induction e as [ | n | e n f He Hf _ (r & Hr) ] using eps0_hnf_pos_rect.
+    + exists 0₀; auto.
+    + exists (eps0_mpos γ n); auto.
+    + exists (eps0_mpos (eps0_momega γ e) n +₀ r); auto.
+  Qed.
+
+  Definition eps0_mult e f := π₁ (eps0_mult_pwc e f).
+
+  Infix "*₀" := eps0_mult.
+
+  Fact eps0_mult_spec e f : eps0_mult_gr e f (e *₀ f).
+  Proof. apply (proj2_sig _). Qed.
+
+  Hint Resolve eps0_mult_spec : core.
+
+  Tactic Notation "solve" "mult" :=
+    intros; apply eps0_mult_fun with (1 := eps0_mult_spec _ _) (3 := eq_refl); auto.
+
+  Fact eps0_mult_zero_right a : a *₀ 0₀ = 0₀.
+  Proof. solve mult. Qed.
+
+  Fact eps0_mult_pos_right a n : a *₀ ω^⟨0₀,n⟩ = eps0_mpos a n.
+  Proof. solve mult. Qed.
+
+  Corollary eps0_mpos_eq a n : eps0_mpos a n = a *₀ ω^⟨0₀,n⟩.
+  Proof. now rewrite eps0_mult_pos_right. Qed.
+
+  Fact eps0_mult_hnf_right a e n f :
+      0₀ <ε₀ e
+    → f <ε₀ ω^e
+    → a *₀ (ω^⟨e,n⟩ +₀ f)
+    = eps0_mpos (eps0_momega a e) n +₀ a *₀ f.
+  Proof. solve mult. Qed.
+
+  (** This one is stronger because it does not need any relation between e and f *)
+  Fact eps0_mult_right a e n f :
+      0₀ <ε₀ e
+    → a *₀ (ω^⟨e,n⟩ +₀ f)
+    = eps0_mpos (eps0_momega a e) n +₀ a *₀ f.
+  Proof.
+    intros He.
+    destruct f as [ | f i g H _ _ ] using eps0_hnf_rect.
+    + rewrite eps0_mult_hnf_right; auto.
+    + destruct (eps0_lt_sdec e f).
+      * rewrite eps0_add_exp_hnf_lt, eps0_mult_hnf_right,
+             <- eps0_add_assoc, eps0_mpos_add_momega; auto.
+        eapply eps0_lt_trans; eassumption.
+      * rewrite eps0_add_exp_hnf_eq, 
+               !eps0_mult_hnf_right,
+             <- eps0_add_assoc,
+                eps0_mpos_add; auto.
+      * rewrite eps0_mult_hnf_right; auto.
+        apply eps0_add_below_omega.
+        - now apply eps0_exp_mono_left.
+        - apply eps0_lt_trans with (1 := H),
+                eps0_omega_mono_lt; auto.
+  Qed.
+
+  Fact eps0_mpos_momega_eq a n e :
+    0₀ <ε₀ e → eps0_mpos (eps0_momega a e) n = a *₀ ω^⟨e,n⟩.
+  Proof.
+    intro.
+    rewrite <- (eps0_add_zero_right ω^⟨_,_⟩),
+                eps0_mult_right,
+                eps0_mult_zero_right,
+                eps0_add_zero_right; auto.
+  Qed.
+
+  Fact eps0_momega_eq a e :
+    0₀ <ε₀ e → eps0_momega a e = a *₀ ω^e.
+  Proof.
+    intro; unfold eps0_omega.
+    rewrite <- eps0_mpos_momega_eq, eps0_mpos_one; auto.
+  Qed.
+
+  Fact eps0_mult_zero_left e : 0₀ *₀ e = 0₀.
+  Proof.
+    induction e as [ | n | e n f He Hf _ IHf ] using eps0_hnf_pos_rect.
+    + now rewrite eps0_mult_zero_right.
+    + now rewrite eps0_mult_pos_right, eps0_mpos_fix_0.
+    + rewrite eps0_mult_hnf_right, IHf; auto.
+      now rewrite eps0_momega_fix_0, eps0_mpos_fix_0, eps0_add_zero_left.
+  Qed.
+
+  Fact eps0_mult_distr a b c : a *₀ (b +₀ c) = a *₀ b +₀ a *₀ c.
+  Proof.
+    induction b as [ | n | e n f He Hf IHe IHf ] in a, c |- *
+      using eps0_hnf_pos_rect.
+    + now rewrite eps0_mult_zero_right, !eps0_add_zero_left.
+    + destruct c as [ | k | c k g ? ? _ _ ] using eps0_hnf_pos_rect.
+      * now rewrite eps0_mult_zero_right, !eps0_add_zero_right.
+      * now rewrite eps0_add_exp, !eps0_mult_pos_right, eps0_mpos_add.
+      * rewrite eps0_add_exp_hnf_lt,
+                eps0_mult_hnf_right,
+                eps0_mult_pos_right,
+             <- eps0_add_assoc,
+                eps0_add_mpos_momega; auto.
+    + rewrite eps0_mult_right,
+             !eps0_add_assoc,
+           <- IHf, eps0_mult_right; auto.
+  Qed.
+
+  Fact eps0_mult_gt_zero a e : 0₀ <ε₀ a → 0₀ <ε₀ e → 0₀ <ε₀ a *₀ e.
+  Proof.
+    intros Ha He.
+    induction e as [ | n | e n f H1 H2 IH1 IH2 ] using eps0_hnf_pos_rect.
+    + now apply eps0_lt_irrefl in He.
+    + rewrite eps0_mult_pos_right; now apply eps0_mpos_gt_zero.
+    + rewrite eps0_mult_right; auto.
+      destruct (eps0_zero_or_pos f) as [ -> | Hf ].
+      * rewrite eps0_mult_zero_right, eps0_add_zero_right.
+        apply eps0_mpos_gt_zero; auto.
+        apply eps0_lt_le_trans with (2 := eps0_momega_lt_pos Ha H1); auto.
+      * apply eps0_lt_le_trans with (1 := IH2 Hf); auto.
+  Qed.
+
+  (* Easy using substraction *)
+  Fact eps0_mult_mono_right a e f :
+    0₀ <ε₀ a → e <ε₀ f → a *₀ e <ε₀ a *₀ f.
+  Proof.
+    intros ? (? & -> & ?)%eps0_lt_inv_add.
+    rewrite eps0_mult_distr.
+    now apply eps0_add_incr, eps0_mult_gt_zero.
+  Qed.
+
+  Fact eps0_mult_mono_left a b e :
+    a <ε₀ b → a *₀ e ≤ε₀ b *₀ e.
+  Proof.
+    intros Hab.
+    induction e as [ | n | e n g H1 IH1 IH2 ] using eps0_hnf_pos_rect.
+    + rewrite !eps0_mult_zero_right; auto.
+    + rewrite !eps0_mult_pos_right.
+      left; apply eps0_mpos_mono_left; auto.
+    + rewrite !eps0_mult_right; auto.
+      apply eps0_add_mono; auto.
+      apply eps0_mpos_mono; auto.
+      apply eps0_momega_mono_left; auto.
+  Qed.
+
+  Fact eps0_mult_mono a b e f :
+    a ≤ε₀ b → e ≤ε₀ f → a *₀ e ≤ε₀ b *₀ f.
+  Proof.
+    destruct (eps0_zero_or_pos a) as [ -> | Ha ].
+    1: rewrite eps0_mult_zero_left; auto.
+    intros [ H1 | <- ] [ H2 | <- ].
+    + apply eps0_le_trans with (a *₀ f).
+      * left; apply eps0_mult_mono_right; auto.
+      * now apply eps0_mult_mono_left.
+    + now apply eps0_mult_mono_left.
+    + left; now apply eps0_mult_mono_right.
+    + now right.
+  Qed.
+
+  Fact eps0_mult_hnf a i b e j f :
+      0₀ <ε₀ e
+    → b <ε₀ ω^a
+    → f <ε₀ ω^e
+    → (ω^⟨a,i⟩ +₀ b) *₀ (ω^⟨e,j⟩ +₀ f)
+     = ω^⟨a+₀e,j⟩ +₀ (ω^⟨a,i⟩ +₀ b) *₀ f.
+  Proof. intros; rewrite eps0_mult_right, eps0_momega_fix_1, eps0_mpos_omega; auto. Qed.
+
+  Fact eps0_mult_hnf_exp a i b e j :
+      0₀ <ε₀ e → b <ε₀ ω^a → (ω^⟨a,i⟩ +₀ b) *₀ ω^⟨e,j⟩ = ω^⟨a+₀e,j⟩.
+  Proof.
+    intros H1 H2.
+    rewrite <- (eps0_add_zero_right ω^⟨_,j⟩), eps0_mult_hnf; auto.
+    now rewrite eps0_mult_zero_right, eps0_add_zero_right.
+  Qed.
+
+  Fact eps0_mult_exp_hnf a i e j f : 
+      0₀ <ε₀ e
+    → f <ε₀ ω^e
+    → ω^⟨a,i⟩ *₀ (ω^⟨e,j⟩ +₀ f)
+    = ω^⟨a+₀e,j⟩ +₀ ω^⟨a,i⟩ *₀ f.
+  Proof. intros; rewrite <- (eps0_add_zero_right ω^⟨_,i⟩), eps0_mult_hnf; auto. Qed.
+
+  Fact eps0_mult_omega_hnf a e j f : 
+      0₀ <ε₀ e
+    → f <ε₀ ω^e
+    → ω^a *₀ (ω^⟨e,j⟩ +₀ f)
+    = ω^⟨a+₀e,j⟩ +₀ ω^a *₀ f.
+  Proof. apply eps0_mult_exp_hnf. Qed.
+
+  Fact eps0_mult_exp_pos e i j : ω^⟨e,i⟩ *₀ ω^⟨0₀,j⟩ = ω^⟨e,i *ₚ j⟩.
+  Proof. now rewrite eps0_mult_pos_right, eps0_mpos_exp. Qed.
+
+  Fact eps0_mult_exp e i f j : 0₀ <ε₀ f → ω^⟨e,i⟩ *₀ ω^⟨f,j⟩ = ω^⟨e+₀f,j⟩.
+  Proof. intro; rewrite <- (eps0_add_zero_right ω^⟨e,i⟩), eps0_mult_hnf_exp; auto. Qed.
+
+  Fact eps0_mult_exp_omega e i f : 0₀ <ε₀ f → ω^⟨e,i⟩ *₀ ω^f = ω^(e+₀f).
+  Proof. intro; apply eps0_mult_exp; auto. Qed.
+
+  Fact eps0_mult_omega_exp e f n: ω^e *₀ ω^⟨f,n⟩ = ω^⟨e+₀f,n⟩.
+  Proof.
+    unfold eps0_omega.
+    destruct (eps0_zero_or_pos f) as [ -> | ].
+    + now rewrite eps0_mult_exp_pos, eps0_add_zero_right.
+    + rewrite eps0_mult_exp; auto.
+  Qed.
+
+  Fact eps0_mult_omega e f : ω^e *₀ ω^f = ω^(e+₀f).
+  Proof. apply eps0_mult_omega_exp. Qed.
+
+  (** From ω^e.n.ω^f = ω^(e+f) *)
+  Fact eps0_mult_below_omega a b e n f : 
+      a <ε₀ ω^⟨e,n⟩
+    → b <ε₀ ω^f
+    → a *₀ b <ε₀ ω^(e+₀f).
+  Proof.
+    intros H1 H2.
+    apply eps0_le_lt_trans with (ω^⟨e,n⟩ *₀ b).
+    + apply eps0_mult_mono; auto.
+    + destruct (eps0_zero_or_pos f) as [ -> | ].
+      * apply eps0_lt_one in H2 as ->.
+        rewrite eps0_mult_zero_right; auto.
+      * rewrite <- eps0_mult_exp_omega with (i := n); auto.
+        apply eps0_mult_mono_right; auto.
+  Qed.
+
+  Remark eps0_mult_below_omega' a b e f : 
+      a <ε₀ ω^e → b <ε₀ ω^f → a *₀ b <ε₀ ω^(e+₀f).
+  Proof. apply eps0_mult_below_omega. Qed.
+
+  Fact eps0_mult_mpos a b n : eps0_mpos (a *₀ b) n = a *₀ eps0_mpos b n. 
+  Proof.
+    induction b using eps0_hnf_pos_rect in a, n |- *.
+    + now rewrite eps0_mult_zero_right, eps0_mpos_fix_0, eps0_mult_zero_right.
+    + now rewrite eps0_mpos_exp, !eps0_mult_pos_right, eps0_mpos_comp.
+    + rewrite eps0_mult_distr.
+      destruct a as [ | ] using eps0_hnf_rect.
+      * now rewrite !eps0_mult_zero_left, eps0_add_zero_left, eps0_mpos_fix_0.
+      * rewrite eps0_mult_hnf_exp, !eps0_mpos_fix_1; auto.
+        - rewrite eps0_mult_distr, eps0_mult_hnf_exp; auto.
+        - apply eps0_mult_below_omega with (n := i0 +ₚ 1ₚ); auto.
+          rewrite <- eps0_add_exp; auto.
+  Qed.
+
+  (** This one was a long shot !! 
+      induction on c and case analysis on b and a *)
+  Theorem eps0_mult_assoc a b c : a *₀ (b *₀ c) = (a *₀ b) *₀ c.
+  Proof.
+    induction c as [ | n | e n f He Hf IHe IHf ]
+      in a, b |- * using eps0_hnf_pos_rect.
+    + now rewrite !eps0_mult_zero_right.
+    + now rewrite !eps0_mult_pos_right, eps0_mult_mpos.
+    + destruct b as [ | i | g i h Hg Hh _ ] using eps0_hnf_pos_rect.
+      * rewrite eps0_mult_zero_left,
+               !eps0_mult_zero_right,
+                eps0_mult_zero_left; auto.
+      * rewrite eps0_mult_exp_hnf,
+                eps0_add_zero_left, 
+               !eps0_mult_distr,
+                IHf,
+                eps0_mult_pos_right,
+            <- !eps0_mpos_momega_eq,
+                eps0_momega_mpos; auto.
+      * rewrite eps0_mult_hnf, eps0_mult_distr, IHf; auto.
+        destruct a as [ | u j v Hu _ _ ] using eps0_hnf_rect.
+        - now rewrite !eps0_mult_zero_left, eps0_add_zero_left.
+        - rewrite eps0_mult_hnf_exp; auto.
+          2: apply eps0_lt_le_trans with (1 := He); auto.
+          rewrite !eps0_mult_hnf, eps0_add_assoc; auto.
+          apply eps0_mult_below_omega with (n := j +ₚ 1ₚ); auto.
+          apply eps0_lt_le_trans with (ω^⟨u,j⟩ +₀ ω^u); auto.
+          unfold eps0_omega; rewrite eps0_add_exp; auto.
+  Qed.
+
+  Fact eps0_mult_one_left e : 1₀ *₀ e = e.
+  Proof.
+    rewrite <- eps0_omega_zero.
+    induction e using eps0_hnf_pos_rect.
+    + now rewrite eps0_mult_zero_right.
+    + now rewrite eps0_mult_pos_right, eps0_mpos_omega.
+    + unfold eps0_omega.
+      rewrite eps0_mult_exp_hnf, eps0_add_zero_left; auto.
+      f_equal; auto.
+  Qed.
+
+  Fact eps0_mult_one_right e : e *₀ 1₀ = e.
+  Proof.
+    rewrite <- eps0_omega_zero; unfold eps0_omega.
+    now rewrite eps0_mult_pos_right, eps0_mpos_one.
+  Qed.
+
+  Fact eps0_mult_zero_inv a e : a *₀ e = 0₀ → a = 0₀ ∨ e = 0₀.
+  Proof.
+    intros E.
+    destruct (eps0_zero_or_pos a) as [ | Ha ]; auto.
+    destruct (eps0_zero_or_pos e) as [ | He ]; auto.
+    destruct (@eps0_lt_irrefl 0₀).
+    rewrite <- E at 2.
+    now apply eps0_mult_gt_zero.
+  Qed.
+
+  Fact eps0_mult_cancel a e f : 0₀ <ε₀ a → a *₀ e = a *₀ f → e = f.
+  Proof.
+    intros Ha H.
+    destruct (eps0_lt_sdec e f) as [ e f C | | e f C ]; auto; exfalso;
+      apply (@eps0_lt_irrefl (a *₀ e)).
+    + rewrite H at 2; now apply eps0_mult_mono_right.
+    + rewrite H at 1; now apply eps0_mult_mono_right.
+  Qed.
+
+  Fact eps0_mult_succ_right a e : a *₀ (S₀ e) = a *₀ e +₀ a.
+  Proof. now rewrite <- eps0_add_one_right, eps0_mult_distr, eps0_mult_one_right. Qed.
+
+End eps0_mult.
+
+Infix "*₀" := eps0_mult.
+
+(* 0.a = a.0 = 0 *)
+Check eps0_mult_zero_left.
+Check eps0_mult_zero_right.
+(* 1.a = a.1 = 0 *)
+Check eps0_mult_one_left.
+Check eps0_mult_one_right.
+(* a.b = 0 → a = 0 ∨ b = 0 *)
+Check eps0_mult_zero_inv.
+(* a.(b.c) = (a.b).c *)
+Check eps0_mult_assoc.
+(* 0 < e -> a < b -> e.a < e.b *)
+Check eps0_mult_mono_right.
+(* Continuity is missing e.(lub P) = lub e.P *)
+Check eps0_mult_mono.
+Check eps0_mult_distr.
+Check eps0_mult_cancel.
+
+(** Section expo *)
+
+Fact eps0_omega_succ e : ω^(S₀ e) = ω^e *₀ ω^1₀.
+Proof.
+  now rewrite <- eps0_succ_zero_is_one,
+                 eps0_mult_omega,
+                 eps0_succ_zero_is_one,
+                 eps0_add_one_right.
+Qed.
+
+Check eps0_omega_zero.
+Check eps0_omega_succ.
+
+Section eps0_exponentiation.
+
+  (** Define exponentiation in CNF 
+   
+      The formula here: 
+
+         https://proofwiki.org/wiki/Ordinal_Exponentiation_via_Cantor_Normal_Form/Limit_Exponents
+
+      (w^a₁.n₁+...+w^aₚ.nₚ)^e = w^(a₁.e) when a₁ > ... > aₚ
+
+      The spec here is probably wrong for α successor
+  *)
+
+  Inductive eps0_expo_gr α : ε₀ → ε₀ → Prop :=
+    | eps0_expr_gr_0 : eps0_expo_gr α 0₀ 0₀
+    | eps0_expr_gr_1 γ n β : β <ε₀ ω^γ → eps0_expo_gr α (ω^⟨γ,n⟩ +₀ β) ω^(γ*₀α).
+
+  Fact eps0_expo_fun α e1 f1 e2 f2 :
+    eps0_expo_gr α e1 f1 → eps0_expo_gr α e2 f2 → e1 = e2 → f1 = f2.
+  Proof.
+    intros [] []; auto.
+    + now intros ?%eps0_zero_neq_hnf.
+    + symm; now intros ?%eps0_zero_neq_hnf.
+    + intros (<- & <- & <-)%eps0_eq_hnf_inv; auto.
+  Qed. 
+
+  Definition eps0_expo_pwc e α : sig (eps0_expo_gr α e).
+  Proof.
+    destruct e as [ | e ] using eps0_hnf_rect.
+    + exists 0₀; constructor.
+    + exists ω^(e*₀α); constructor; auto.
+  Qed.
+
+  Definition eps0_expo e α := proj1_sig (eps0_expo_pwc e α).
+
+  Fact eps0_expo_spec e α : eps0_expo_gr α e (eps0_expo e α).
+  Proof. apply (proj2_sig _). Qed.
+
+  Hint Constructors eps0_expo_gr : core.
+  Hint Resolve eps0_expo_spec : core.
+
+  Tactic Notation "functionality" :=
+    apply eps0_expo_fun with (1 := eps0_expo_spec _ _) (3 := eq_refl); auto.
+
+  Fact eps0_expo_zero e : eps0_expo 0₀ e = 0₀.
+  Proof. functionality; constructor. Qed.
+
+  Fact eps0_expo_head a n b e : b <ε₀ ω^a → eps0_expo (ω^⟨a,n⟩ +₀ b) e = ω^(a*₀e).
+  Proof. intros; functionality; constructor; auto. Qed.
+
+  Fact eps0_expo_exp_S a n e : eps0_expo ω^⟨a,n⟩ e = ω^(a*₀e).
+  Proof. rewrite <- (eps0_add_zero_right ω^⟨_,n⟩), eps0_expo_head; auto. Qed.
+
+  Fact eps0_expo_omega_pos n e : eps0_expo ω^⟨1₀,n⟩ e = ω^e.
+  Proof. now rewrite eps0_expo_exp_S, eps0_mult_one_left. Qed.
+
+  Fact eps0_expo_omega a e : eps0_expo ω^a e = ω^(a*₀e).
+  Proof. apply eps0_expo_exp_S. Qed.
+
+  (** Need to check more equations *)
+
+End eps0_exponentiation.
+
+
