theories/fgh.v
@@ -8,7 +8,7 @@
 (**************************************************************)
 
 From Coq Require Import List Relations Arith Lia Wellfounded Utf8.
-From Hydra Require Import utils pos eps0 eps0_least_split eps0_fseq.
+From Hydra Require Import utils pos eps0 eps0_ltf eps0_fseq.
 
 Set Implicit Arguments.
 
@@ -21,9 +21,9 @@ Section Fast_Growing_Hierarchy.
 
       F 0₀ n      := S n             for 0₀
       F (S₀ e) n  := (F e)^{S n} n   for a successor ordinal
-      F λ n       := F λ[n] n        for a limit ordinal, using the fund. seq. λ[_]
+      F λ n       := F λ[n] n        for a limit ordinal λ, using the fund. seq. λ[_]
 
-      We specify it as a relation between ε₀ and nat → nat
+      We specify it as a relation between the types ε₀ and (nat → nat)
 
   *)
 
@@ -35,6 +35,8 @@ Section Fast_Growing_Hierarchy.
                      → fgh_gr e (λ n, F n n).
 
   Hint Constructors fgh_gr : core.
+
+  Hint Resolve eps0_is_succ_S : core.
 
   Lemma fgh_gr_fun e E f F : fgh_gr e E → fgh_gr f F → e = f → ∀n, E n = F n.
   Proof.
@@ -58,15 +60,15 @@ Section Fast_Growing_Hierarchy.
     | eps0_choice_2 e : eps0_is_limit e
                       → eps0_choice e.
 
-  Hint Resolve eps0_lt_succ eps0_is_limit_omega eps0_is_limit_add_omega : core.
+  Hint Resolve eps0_lt_succ eps0_is_limit_omega eps0_is_limit_tf : core.
 
   Fact eps0_choose e : eps0_choice e.
-  Proof. induction e using eps0_tail_rect; constructor; auto. Qed.
+  Proof. induction e using eps0_ltf_pos_rect; constructor; auto. Qed.
 
   (** This is the Grzegorczyk hierarchy *)
   Definition FGH_pwc e : { F | fgh_gr e F }.
   Proof.
-    induction e as [ e IH ] using (well_founded_induction_type wf_eps0_lt).
+    induction e as [ e IH ] using eps0_rect.
     destruct (eps0_choose e) as [ | e | e l ].
     + exists S; auto.
     + destruct (IH e) as (F & ?); auto.
@@ -74,11 +76,11 @@ Section Fast_Growing_Hierarchy.
     + set (F i := π₁ (IH (eps0_fseq l i) (eps0_fseq_lt _ _))).
       exists (λ n, F n n).
       constructor 3 with l.
-      intro; apply (proj2_sig (IH (eps0_fseq l n) (eps0_fseq_lt _ _))).
+      intro; apply (π₂ (IH (eps0_fseq l n) (eps0_fseq_lt _ _))).
   Qed.
 
   (* The hierarchy is uniquely characterized, up to extensionality 
-     provided the fundemental sequence is uniquely characterized 
+     provided the fundamental sequence is uniquely characterized 
      as well !! *)
 
   Definition FGH e := π₁ (FGH_pwc e). 
@@ -90,23 +92,27 @@ Section Fast_Growing_Hierarchy.
 
   (** We establish the defining equations using the spec *)
 
-  Tactic Notation "functionality" :=
+  Tactic Notation "solve" "fgh" :=
     apply fgh_gr_fun with (1 := FGH_spec _) (3 := eq_refl); eauto.
 
   Theorem FGH_fix_zero n : FGH 0₀ n = S n.
-  Proof. functionality. Qed. 
+  Proof. solve fgh. Qed. 
 
   Theorem FGH_fix_succ e n : FGH (S₀ e) n = iter (FGH e) (S n) n.
   Proof.
     change (FGH (S₀ e) n = (λ n, iter (FGH e) (S n) n) n).
-    functionality.
+    solve fgh.
   Qed.
 
   Theorem FGH_fix_limit e l n : FGH e n = FGH (@eps0_fseq e l n) n.
   Proof.
     change (FGH e n = (λ n, FGH (@eps0_fseq e l n) n) n).
-    functionality.
+    solve fgh.
     constructor 3 with l; auto.
   Qed.
 
 End Fast_Growing_Hierarchy.
+
+Check FGH_fix_zero.
+Check FGH_fix_succ.
+Check FGH_fix_limit.
